<?xml version="1.0"?>
<rdf:RDF xmlns="http://www.kracr.iiitd.edu.in/ontology/apple#"
     xml:base="http://www.kracr.iiitd.edu.in/ontology/apple"
     xmlns:owl="http://www.w3.org/2002/07/owl#"
     xmlns:rdf="http://www.w3.org/1999/02/22-rdf-syntax-ns#"
     xmlns:xml="http://www.w3.org/XML/1998/namespace"
     xmlns:xsd="http://www.w3.org/2001/XMLSchema#"
     xmlns:AIRO="https://w3id.org/AIRO#"
     xmlns:rdfs="http://www.w3.org/2000/01/rdf-schema#"
     xmlns:swrl="http://www.w3.org/2003/11/swrl#"
     xmlns:time="http://www.w3.org/2006/time#"
     xmlns:apple="http://www.kracr.iiitd.edu.in/ontology/apple/"
     xmlns:event="http://w3id.org/daselab/onto/event#"
     xmlns:swrlb="http://www.w3.org/2003/11/swrlb#"
     xmlns:terms="http://purl.org/dc/terms/"
     xmlns:traffic="http://www.sensormeasurement.appspot.com/ont/transport/traffic#"
     xmlns:objectrole="http://www.ontologydesignpatterns.org/cp/owl/objectrole.owl#"
     xmlns:trajectory="http://w3id.org/daselab/onto/trajectory#"
     xmlns:participation="http://www.ontologydesignpatterns.org/cp/owl/participation.owl#"
     xmlns:coparticipation="http://www.ontologydesignpatterns.org/cp/owl/coparticipation.owl#">
    <owl:Ontology rdf:about="http://www.kracr.iiitd.edu.in/ontology/apple">
        <owl:versionIRI rdf:resource="http://www.kracr.iiitd.edu.in/ontology/apple/1.0"/>
        <terms:contributor rdf:datatype="http://www.w3.org/2001/XMLSchema#string">Manohar Kumar</terms:contributor>
        <terms:creator rdf:datatype="http://www.w3.org/2001/XMLSchema#string">Aisha Aijaz</terms:creator>
        <terms:creator rdf:datatype="http://www.w3.org/2001/XMLSchema#string">Raghava Mutharaju</terms:creator>
        <terms:description rdf:datatype="http://www.w3.org/2001/XMLSchema#string">An Ontology for applied ethics and context to capture relevant ethical information that may provide insight to the morality of a course of action during a particular event.</terms:description>
        <terms:title rdf:datatype="http://www.w3.org/2001/XMLSchema#string">ApplE: An Applied Ethics Ontology</terms:title>
        <owl:versionInfo rdf:datatype="http://www.w3.org/2001/XMLSchema#string">Version 1.0 of the ApplE Ontology for Applied Ethics.</owl:versionInfo>
    </owl:Ontology>
    


    <!-- 
    ///////////////////////////////////////////////////////////////////////////////////////
    //
    // Annotation properties
    //
    ///////////////////////////////////////////////////////////////////////////////////////
     -->

    


    <!-- http://purl.org/dc/terms/contributor -->

    <owl:AnnotationProperty rdf:about="http://purl.org/dc/terms/contributor"/>
    


    <!-- http://purl.org/dc/terms/creator -->

    <owl:AnnotationProperty rdf:about="http://purl.org/dc/terms/creator"/>
    


    <!-- http://purl.org/dc/terms/description -->

    <owl:AnnotationProperty rdf:about="http://purl.org/dc/terms/description"/>
    


    <!-- http://purl.org/dc/terms/title -->

    <owl:AnnotationProperty rdf:about="http://purl.org/dc/terms/title"/>
    


    <!-- 
    ///////////////////////////////////////////////////////////////////////////////////////
    //
    // Object Properties
    //
    ///////////////////////////////////////////////////////////////////////////////////////
     -->

    


    <!-- http://w3id.org/daselab/onto/event#hasInformationObject -->

    <owl:ObjectProperty rdf:about="http://w3id.org/daselab/onto/event#hasInformationObject">
        <owl:inverseOf rdf:resource="http://www.kracr.iiitd.edu.in/ontology/apple/occursInEvent"/>
        <rdfs:domain rdf:resource="http://schema.org/Event"/>
        <rdfs:range rdf:resource="http://schema.mobivoc.org/Action"/>
        <rdfs:comment>Property relating Event to InformationObject in this pattern. The domain of this property is not restricted to Event  since it is possible that non-event to have an information object. The range is always InformationObject since it makes no sense to have a property named hasInformationObject to point to anything other than information object.

However, when reusing this concept from the EventCore ODP for the ApplE ontology, this property will link an event and an action.</rdfs:comment>
    </owl:ObjectProperty>
    


    <!-- http://w3id.org/daselab/onto/event#subEventOf -->

    <owl:ObjectProperty rdf:about="http://w3id.org/daselab/onto/event#subEventOf">
        <rdf:type rdf:resource="http://www.w3.org/2002/07/owl#SymmetricProperty"/>
        <rdf:type rdf:resource="http://www.w3.org/2002/07/owl#TransitiveProperty"/>
        <rdfs:domain rdf:resource="http://schema.org/Event"/>
        <rdfs:range rdf:resource="http://schema.org/Event"/>
        <rdfs:comment>Property expressing partonomic relation between two events. Domain and range are always Event.</rdfs:comment>
    </owl:ObjectProperty>
    


    <!-- http://w3id.org/daselab/onto/trajectory#atPlace -->

    <owl:ObjectProperty rdf:about="http://w3id.org/daselab/onto/trajectory#atPlace">
        <rdf:type rdf:resource="http://www.w3.org/2002/07/owl#AsymmetricProperty"/>
        <rdf:type rdf:resource="http://www.w3.org/2002/07/owl#IrreflexiveProperty"/>
        <rdfs:domain rdf:resource="http://schema.org/Event"/>
        <rdfs:range rdf:resource="http://w3id.org/daselab/onto/trajectory#Place"/>
        <rdfs:comment>A property that describes where an action occurred.</rdfs:comment>
    </owl:ObjectProperty>
    


    <!-- http://w3id.org/daselab/onto/trajectory#atTime -->

    <owl:ObjectProperty rdf:about="http://w3id.org/daselab/onto/trajectory#atTime">
        <rdf:type rdf:resource="http://www.w3.org/2002/07/owl#AsymmetricProperty"/>
        <rdf:type rdf:resource="http://www.w3.org/2002/07/owl#IrreflexiveProperty"/>
        <rdfs:domain rdf:resource="http://schema.org/Event"/>
        <rdfs:range rdf:resource="http://w3id.org/daselab/onto/trajectory#TimeEntity"/>
        <rdfs:comment>A property that describes when an action occurred.</rdfs:comment>
    </owl:ObjectProperty>
    


    <!-- http://www.kracr.iiitd.edu.in/ontology/apple#describedBy -->

    <owl:ObjectProperty rdf:about="http://www.kracr.iiitd.edu.in/ontology/apple#describedBy">
        <rdfs:subPropertyOf rdf:resource="http://www.w3.org/2002/07/owl#topObjectProperty"/>
        <owl:inverseOf rdf:resource="http://www.kracr.iiitd.edu.in/ontology/apple/describesEvent"/>
        <rdfs:domain rdf:resource="http://schema.org/Event"/>
        <rdfs:range rdf:resource="http://contextus.net/ontology/ontomedia/core/expression#Context"/>
    </owl:ObjectProperty>
    


    <!-- http://www.kracr.iiitd.edu.in/ontology/apple#hasDurationOfConsequence -->

    <owl:ObjectProperty rdf:about="http://www.kracr.iiitd.edu.in/ontology/apple#hasDurationOfConsequence">
        <rdfs:subPropertyOf rdf:resource="http://www.kracr.iiitd.edu.in/ontology/apple/hasCharacteristicOfConsequence"/>
        <rdfs:domain rdf:resource="https://w3id.org/AIRO#Consequence"/>
        <rdfs:range rdf:resource="http://www.kracr.iiitd.edu.in/ontology/apple/DurationOfConsequence"/>
    </owl:ObjectProperty>
    


    <!-- http://www.kracr.iiitd.edu.in/ontology/apple#hasSeverityOfConsequence -->

    <owl:ObjectProperty rdf:about="http://www.kracr.iiitd.edu.in/ontology/apple#hasSeverityOfConsequence">
        <rdfs:subPropertyOf rdf:resource="http://www.kracr.iiitd.edu.in/ontology/apple/hasCharacteristicOfConsequence"/>
        <rdfs:domain rdf:resource="https://w3id.org/AIRO#Consequence"/>
        <rdfs:range rdf:resource="http://www.kracr.iiitd.edu.in/ontology/apple/SeverityOfConsequence"/>
    </owl:ObjectProperty>
    


    <!-- http://www.kracr.iiitd.edu.in/ontology/apple#hasUtilityOfConsequence -->

    <owl:ObjectProperty rdf:about="http://www.kracr.iiitd.edu.in/ontology/apple#hasUtilityOfConsequence">
        <rdfs:subPropertyOf rdf:resource="http://www.kracr.iiitd.edu.in/ontology/apple/hasCharacteristicOfConsequence"/>
        <rdfs:domain rdf:resource="https://w3id.org/AIRO#Consequence"/>
        <rdfs:range rdf:resource="http://www.kracr.iiitd.edu.in/ontology/apple/UtilityOfConsequence"/>
    </owl:ObjectProperty>
    


    <!-- http://www.kracr.iiitd.edu.in/ontology/apple#violatedByAction -->

    <owl:ObjectProperty rdf:about="http://www.kracr.iiitd.edu.in/ontology/apple#violatedByAction">
        <owl:inverseOf rdf:resource="http://www.kracr.iiitd.edu.in/ontology/apple/violatesEthicalPrinciple"/>
        <rdfs:domain rdf:resource="http://www.kracr.iiitd.edu.in/ontology/apple/EthicalPrinciple"/>
        <rdfs:range rdf:resource="http://schema.mobivoc.org/Action"/>
        <rdfs:comment>This property describes the ethical principle that was violated by the occurrence of an action.</rdfs:comment>
    </owl:ObjectProperty>
    


    <!-- http://www.kracr.iiitd.edu.in/ontology/apple/adheresTo -->

    <owl:ObjectProperty rdf:about="http://www.kracr.iiitd.edu.in/ontology/apple/adheresTo">
        <owl:inverseOf rdf:resource="http://www.kracr.iiitd.edu.in/ontology/apple/appliesTo"/>
        <rdf:type rdf:resource="http://www.w3.org/2002/07/owl#FunctionalProperty"/>
        <rdf:type rdf:resource="http://www.w3.org/2002/07/owl#AsymmetricProperty"/>
        <rdf:type rdf:resource="http://www.w3.org/2002/07/owl#IrreflexiveProperty"/>
        <rdfs:domain rdf:resource="https://w3id.org/AIRO#Domain"/>
        <rdfs:range rdf:resource="http://www.kracr.iiitd.edu.in/ontology/apple/AppliedEthics"/>
        <rdfs:comment>A domain adheres to a specific type of applied ethics. For example, the medical domain adheres to bioethics. Again, this connection is not absolute. For example, an issue of the medical domain may also require adherance to the professional domain, when considering the treatment of nurses and doctors in large private hospitals.</rdfs:comment>
    </owl:ObjectProperty>
    


    <!-- http://www.kracr.iiitd.edu.in/ontology/apple/affects -->

    <owl:ObjectProperty rdf:about="http://www.kracr.iiitd.edu.in/ontology/apple/affects">
        <rdf:type rdf:resource="http://www.w3.org/2002/07/owl#AsymmetricProperty"/>
        <rdf:type rdf:resource="http://www.w3.org/2002/07/owl#IrreflexiveProperty"/>
        <rdfs:domain rdf:resource="http://schema.mobivoc.org/Action"/>
        <rdfs:range rdf:resource="http://www.kracr.iiitd.edu.in/ontology/apple/PassiveAgent"/>
        <rdfs:comment>Affects implies the verb in the statement &quot;an action affects a passive agent&quot; in whatever way, shape, or form.</rdfs:comment>
    </owl:ObjectProperty>
    


    <!-- http://www.kracr.iiitd.edu.in/ontology/apple/appliesPhilosophy -->

    <owl:ObjectProperty rdf:about="http://www.kracr.iiitd.edu.in/ontology/apple/appliesPhilosophy">
        <rdf:type rdf:resource="http://www.w3.org/2002/07/owl#AsymmetricProperty"/>
        <rdf:type rdf:resource="http://www.w3.org/2002/07/owl#IrreflexiveProperty"/>
        <rdfs:domain rdf:resource="http://www.kracr.iiitd.edu.in/ontology/apple/AppliedEthics"/>
        <rdfs:range rdf:resource="http://www.kracr.iiitd.edu.in/ontology/apple/AppliedEthicsPhilosophy"/>
        <rdfs:comment>A type of applied ethics may apply a type of philosophy.</rdfs:comment>
    </owl:ObjectProperty>
    


    <!-- http://www.kracr.iiitd.edu.in/ontology/apple/appliesTo -->

    <owl:ObjectProperty rdf:about="http://www.kracr.iiitd.edu.in/ontology/apple/appliesTo">
        <rdfs:domain rdf:resource="http://www.kracr.iiitd.edu.in/ontology/apple/AppliedEthics"/>
        <rdfs:range rdf:resource="https://w3id.org/AIRO#Domain"/>
        <rdfs:comment>Inverse of the adheresTo object property. This property implies that a type of applied ethics applies to a certain domain.</rdfs:comment>
    </owl:ObjectProperty>
    


    <!-- http://www.kracr.iiitd.edu.in/ontology/apple/associatedWith -->

    <owl:ObjectProperty rdf:about="http://www.kracr.iiitd.edu.in/ontology/apple/associatedWith">
        <rdf:type rdf:resource="http://www.w3.org/2002/07/owl#AsymmetricProperty"/>
        <rdf:type rdf:resource="http://www.w3.org/2002/07/owl#IrreflexiveProperty"/>
        <rdfs:domain rdf:resource="http://www.kracr.iiitd.edu.in/ontology/apple/NormativeEthics"/>
        <rdfs:range rdf:resource="http://www.kracr.iiitd.edu.in/ontology/apple/EthicalPrinciple"/>
        <rdfs:comment>Types of normative ethics may be associated with certain ethical concepts.</rdfs:comment>
    </owl:ObjectProperty>
    


    <!-- http://www.kracr.iiitd.edu.in/ontology/apple/causesEthicalIssue -->

    <owl:ObjectProperty rdf:about="http://www.kracr.iiitd.edu.in/ontology/apple/causesEthicalIssue">
        <rdf:type rdf:resource="http://www.w3.org/2002/07/owl#AsymmetricProperty"/>
        <rdf:type rdf:resource="http://www.w3.org/2002/07/owl#IrreflexiveProperty"/>
        <rdfs:domain rdf:resource="https://w3id.org/AIRO#Consequence"/>
        <rdfs:range rdf:resource="http://www.kracr.iiitd.edu.in/ontology/apple/EthicalIssue"/>
        <rdfs:comment>The consequence of an action may cause an ethical issue. (This is not to be confused with the fact that some may consider a consequence to be an ethical issue, as these are two separate concepts. For example: the firing of an employee on the basis of their race is a consequence of the &apos;firing&apos; action. However, the firing is not the ethical issue. The issue is a business ethical issue: Discrimination in the workplace.)</rdfs:comment>
    </owl:ObjectProperty>
    


    <!-- http://www.kracr.iiitd.edu.in/ontology/apple/describesEvent -->

    <owl:ObjectProperty rdf:about="http://www.kracr.iiitd.edu.in/ontology/apple/describesEvent">
        <rdf:type rdf:resource="http://www.w3.org/2002/07/owl#AsymmetricProperty"/>
        <rdf:type rdf:resource="http://www.w3.org/2002/07/owl#IrreflexiveProperty"/>
        <rdfs:domain rdf:resource="http://contextus.net/ontology/ontomedia/core/expression#Context"/>
        <rdfs:range rdf:resource="http://schema.org/Event"/>
        <rdfs:comment>The context describes an event that has occured.</rdfs:comment>
    </owl:ObjectProperty>
    


    <!-- http://www.kracr.iiitd.edu.in/ontology/apple/hasCharacteristicOfConsequence -->

    <owl:ObjectProperty rdf:about="http://www.kracr.iiitd.edu.in/ontology/apple/hasCharacteristicOfConsequence">
        <rdf:type rdf:resource="http://www.w3.org/2002/07/owl#AsymmetricProperty"/>
        <rdf:type rdf:resource="http://www.w3.org/2002/07/owl#IrreflexiveProperty"/>
        <rdfs:domain rdf:resource="https://w3id.org/AIRO#Consequence"/>
        <rdfs:range rdf:resource="http://www.kracr.iiitd.edu.in/ontology/apple/CharacteristicOfConsequence"/>
        <rdfs:comment>This object property describes the characteristic of the consequences of an action.</rdfs:comment>
    </owl:ObjectProperty>
    


    <!-- http://www.kracr.iiitd.edu.in/ontology/apple/hasMoralIntention -->

    <owl:ObjectProperty rdf:about="http://www.kracr.iiitd.edu.in/ontology/apple/hasMoralIntention">
        <rdf:type rdf:resource="http://www.w3.org/2002/07/owl#AsymmetricProperty"/>
        <rdf:type rdf:resource="http://www.w3.org/2002/07/owl#IrreflexiveProperty"/>
        <rdfs:domain rdf:resource="http://www.kracr.iiitd.edu.in/ontology/apple/ActiveAgent"/>
        <rdfs:range rdf:resource="http://www.kracr.iiitd.edu.in/ontology/apple/MoralIntention"/>
        <rdfs:comment>An agent, when doing an action, has moral intention behind the action.</rdfs:comment>
    </owl:ObjectProperty>
    


    <!-- http://www.kracr.iiitd.edu.in/ontology/apple/occursInDomain -->

    <owl:ObjectProperty rdf:about="http://www.kracr.iiitd.edu.in/ontology/apple/occursInDomain">
        <rdfs:subPropertyOf rdf:resource="http://www.w3.org/2002/07/owl#topObjectProperty"/>
        <rdf:type rdf:resource="http://www.w3.org/2002/07/owl#FunctionalProperty"/>
        <rdf:type rdf:resource="http://www.w3.org/2002/07/owl#AsymmetricProperty"/>
        <rdf:type rdf:resource="http://www.w3.org/2002/07/owl#IrreflexiveProperty"/>
        <rdfs:domain rdf:resource="http://schema.org/Event"/>
        <rdfs:range rdf:resource="https://w3id.org/AIRO#Domain"/>
        <rdfs:comment>An event occurs in some domain.</rdfs:comment>
    </owl:ObjectProperty>
    


    <!-- http://www.kracr.iiitd.edu.in/ontology/apple/occursInEvent -->

    <owl:ObjectProperty rdf:about="http://www.kracr.iiitd.edu.in/ontology/apple/occursInEvent">
        <rdf:type rdf:resource="http://www.w3.org/2002/07/owl#AsymmetricProperty"/>
        <rdf:type rdf:resource="http://www.w3.org/2002/07/owl#IrreflexiveProperty"/>
        <rdfs:domain rdf:resource="http://schema.mobivoc.org/Action"/>
        <rdfs:range rdf:resource="http://schema.org/Event"/>
        <rdfs:comment>An action occurs during some event.</rdfs:comment>
    </owl:ObjectProperty>
    


    <!-- http://www.kracr.iiitd.edu.in/ontology/apple/resolvedBy -->

    <owl:ObjectProperty rdf:about="http://www.kracr.iiitd.edu.in/ontology/apple/resolvedBy">
        <owl:inverseOf rdf:resource="http://www.kracr.iiitd.edu.in/ontology/apple/resolves"/>
        <rdf:type rdf:resource="http://www.w3.org/2002/07/owl#AsymmetricProperty"/>
        <rdf:type rdf:resource="http://www.w3.org/2002/07/owl#IrreflexiveProperty"/>
        <rdfs:domain rdf:resource="http://www.kracr.iiitd.edu.in/ontology/apple/EthicalIssue"/>
        <rdfs:range rdf:resource="http://www.kracr.iiitd.edu.in/ontology/apple/AppliedEthicsPhilosophy"/>
        <rdfs:comment>An ethical issue is resolved by an applied ethics philosophy. Here &apos;resolves&apos; implies the resolution of the issue.</rdfs:comment>
    </owl:ObjectProperty>
    


    <!-- http://www.kracr.iiitd.edu.in/ontology/apple/resolves -->

    <owl:ObjectProperty rdf:about="http://www.kracr.iiitd.edu.in/ontology/apple/resolves">
        <rdfs:domain rdf:resource="http://www.kracr.iiitd.edu.in/ontology/apple/AppliedEthicsPhilosophy"/>
        <rdfs:range rdf:resource="http://www.kracr.iiitd.edu.in/ontology/apple/EthicalIssue"/>
        <rdfs:comment>Inverse of the resolvedBy property. An applied ethics philosophy resolves an applied ethics issue. Although the term is assertive (resolves), the property demostrates that a certain property may be used to resolve an ethical issue.</rdfs:comment>
    </owl:ObjectProperty>
    


    <!-- http://www.kracr.iiitd.edu.in/ontology/apple/upholdsEthicalPrinciple -->

    <owl:ObjectProperty rdf:about="http://www.kracr.iiitd.edu.in/ontology/apple/upholdsEthicalPrinciple">
        <rdfs:subPropertyOf rdf:resource="http://www.w3.org/2002/07/owl#topObjectProperty"/>
        <rdf:type rdf:resource="http://www.w3.org/2002/07/owl#AsymmetricProperty"/>
        <rdf:type rdf:resource="http://www.w3.org/2002/07/owl#IrreflexiveProperty"/>
        <rdfs:domain rdf:resource="http://schema.mobivoc.org/Action"/>
        <rdfs:range rdf:resource="http://www.kracr.iiitd.edu.in/ontology/apple/EthicalPrinciple"/>
        <rdfs:comment>An action may uphold certain ethical principles.</rdfs:comment>
    </owl:ObjectProperty>
    


    <!-- http://www.kracr.iiitd.edu.in/ontology/apple/violatesEthicalPrinciple -->

    <owl:ObjectProperty rdf:about="http://www.kracr.iiitd.edu.in/ontology/apple/violatesEthicalPrinciple">
        <rdf:type rdf:resource="http://www.w3.org/2002/07/owl#AsymmetricProperty"/>
        <rdf:type rdf:resource="http://www.w3.org/2002/07/owl#IrreflexiveProperty"/>
        <rdfs:domain rdf:resource="http://schema.mobivoc.org/Action"/>
        <rdfs:range rdf:resource="http://www.kracr.iiitd.edu.in/ontology/apple/EthicalPrinciple"/>
        <rdfs:comment>An action may violate certain ethical principles.</rdfs:comment>
    </owl:ObjectProperty>
    


    <!-- http://www.ontologydesignpatterns.org/cp/owl/coparticipation.owl#coparticipatesWith -->

    <owl:ObjectProperty rdf:about="http://www.ontologydesignpatterns.org/cp/owl/coparticipation.owl#coparticipatesWith">
        <rdf:type rdf:resource="http://www.w3.org/2002/07/owl#SymmetricProperty"/>
        <rdfs:domain rdf:resource="http://xmlns.com/foaf/0.1/Agent"/>
        <rdfs:range rdf:resource="http://xmlns.com/foaf/0.1/Agent"/>
        <rdfs:comment>Agents may co-participate with each other in an event in any capacity (active or passive).</rdfs:comment>
        <rdfs:isDefinedBy>http://www.ontologydesignpatterns.org/cp/owl/coparticipation.owl#</rdfs:isDefinedBy>
    </owl:ObjectProperty>
    


    <!-- http://www.ontologydesignpatterns.org/cp/owl/objectrole.owl#hasRole -->

    <owl:ObjectProperty rdf:about="http://www.ontologydesignpatterns.org/cp/owl/objectrole.owl#hasRole">
        <owl:inverseOf rdf:resource="http://www.ontologydesignpatterns.org/cp/owl/objectrole.owl#isRoleOf"/>
        <rdfs:domain rdf:resource="http://xmlns.com/foaf/0.1/Agent"/>
        <rdfs:range rdf:resource="http://www.ontologydesignpatterns.org/cp/owl/objectrole.owl#Role"/>
        <rdfs:comment>A relation between an object and a role, e.g. the person &apos;John&apos; has role &apos;student&apos;.</rdfs:comment>
        <rdfs:isDefinedBy>http://www.ontologydesignpatterns.org/cp/owl/objectrole.owl</rdfs:isDefinedBy>
    </owl:ObjectProperty>
    


    <!-- http://www.ontologydesignpatterns.org/cp/owl/objectrole.owl#isRoleOf -->

    <owl:ObjectProperty rdf:about="http://www.ontologydesignpatterns.org/cp/owl/objectrole.owl#isRoleOf">
        <rdfs:domain rdf:resource="http://www.ontologydesignpatterns.org/cp/owl/objectrole.owl#Role"/>
        <rdfs:range rdf:resource="http://xmlns.com/foaf/0.1/Agent"/>
        <rdfs:comment>A relation between an object and a role, e.g. the &apos;student&apos; is the role of &apos;John&apos;.</rdfs:comment>
        <rdfs:isDefinedBy>http://www.ontologydesignpatterns.org/cp/owl/objectrole.owl</rdfs:isDefinedBy>
    </owl:ObjectProperty>
    


    <!-- http://www.ontologydesignpatterns.org/cp/owl/participation.owl#hasParticipant -->

    <owl:ObjectProperty rdf:about="http://www.ontologydesignpatterns.org/cp/owl/participation.owl#hasParticipant">
        <owl:inverseOf rdf:resource="http://www.ontologydesignpatterns.org/cp/owl/participation.owl#isParticipantIn"/>
        <rdf:type rdf:resource="http://www.w3.org/2002/07/owl#AsymmetricProperty"/>
        <rdf:type rdf:resource="http://www.w3.org/2002/07/owl#IrreflexiveProperty"/>
        <rdfs:domain rdf:resource="http://schema.org/Event"/>
        <rdfs:range rdf:resource="http://xmlns.com/foaf/0.1/Agent"/>
        <rdfs:comment>Inverse of the &quot;isParticipantIn&quot; object property from the participant Ontology Design Pattern. Shows an event which has a participating agent.</rdfs:comment>
        <rdfs:isDefinedBy>http://www.ontologydesignpatterns.org/cp/owl/participation.owl#</rdfs:isDefinedBy>
    </owl:ObjectProperty>
    


    <!-- http://www.ontologydesignpatterns.org/cp/owl/participation.owl#isParticipantIn -->

    <owl:ObjectProperty rdf:about="http://www.ontologydesignpatterns.org/cp/owl/participation.owl#isParticipantIn">
        <rdf:type rdf:resource="http://www.w3.org/2002/07/owl#AsymmetricProperty"/>
        <rdf:type rdf:resource="http://www.w3.org/2002/07/owl#IrreflexiveProperty"/>
        <rdfs:domain rdf:resource="http://xmlns.com/foaf/0.1/Agent"/>
        <rdfs:range rdf:resource="http://schema.org/Event"/>
        <rdfs:comment>An agent is a participant in an event.</rdfs:comment>
        <rdfs:isDefinedBy>http://www.ontologydesignpatterns.org/cp/owl/participation.owl#</rdfs:isDefinedBy>
    </owl:ObjectProperty>
    


    <!-- http://www.sensormeasurement.appspot.com/ont/transport/traffic#doesAction -->

    <owl:ObjectProperty rdf:about="http://www.sensormeasurement.appspot.com/ont/transport/traffic#doesAction">
        <rdf:type rdf:resource="http://www.w3.org/2002/07/owl#AsymmetricProperty"/>
        <rdf:type rdf:resource="http://www.w3.org/2002/07/owl#IrreflexiveProperty"/>
        <rdfs:domain rdf:resource="http://www.kracr.iiitd.edu.in/ontology/apple/ActiveAgent"/>
        <rdfs:range rdf:resource="http://schema.mobivoc.org/Action"/>
        <rdfs:comment>Doing an action. 
This property describes the relationship between an active agent and the action they do.</rdfs:comment>
    </owl:ObjectProperty>
    


    <!-- https://w3id.org/AIRO#hasConsequence -->

    <owl:ObjectProperty rdf:about="https://w3id.org/AIRO#hasConsequence">
        <rdf:type rdf:resource="http://www.w3.org/2002/07/owl#AsymmetricProperty"/>
        <rdf:type rdf:resource="http://www.w3.org/2002/07/owl#IrreflexiveProperty"/>
        <rdfs:domain rdf:resource="http://schema.mobivoc.org/Action"/>
        <rdfs:range rdf:resource="https://w3id.org/AIRO#Consequence"/>
        <rdfs:comment>An action has a consequence.</rdfs:comment>
    </owl:ObjectProperty>
    


    <!-- 
    ///////////////////////////////////////////////////////////////////////////////////////
    //
    // Data properties
    //
    ///////////////////////////////////////////////////////////////////////////////////////
     -->

    


    <!-- http://www.kracr.iiitd.edu.in/ontology/apple/hasScore -->

    <owl:DatatypeProperty rdf:about="http://www.kracr.iiitd.edu.in/ontology/apple/hasScore">
        <rdfs:domain rdf:resource="http://www.kracr.iiitd.edu.in/ontology/apple/CharacteristicOfConsequence"/>
        <rdfs:range rdf:resource="http://www.w3.org/2001/XMLSchema#integer"/>
        <owl:propertyDisjointWith rdf:resource="http://www.w3.org/2006/time#hasBeginning"/>
        <owl:propertyDisjointWith rdf:resource="http://www.w3.org/2006/time#hasEnd"/>
        <rdfs:comment>Provides a descriptive value to the important factors we have considered that help to make a decision regarding the morality of an action.</rdfs:comment>
    </owl:DatatypeProperty>
    


    <!-- http://www.w3.org/2006/time#hasBeginning -->

    <owl:DatatypeProperty rdf:about="http://www.w3.org/2006/time#hasBeginning">
        <rdfs:domain rdf:resource="http://w3id.org/daselab/onto/trajectory#TimeEntity"/>
        <rdfs:range rdf:resource="http://www.w3.org/2001/XMLSchema#dateTime"/>
        <rdfs:comment>A data property reused from the time ODP and describes when an event begins to occur.</rdfs:comment>
    </owl:DatatypeProperty>
    


    <!-- http://www.w3.org/2006/time#hasEnd -->

    <owl:DatatypeProperty rdf:about="http://www.w3.org/2006/time#hasEnd">
        <rdfs:domain rdf:resource="http://w3id.org/daselab/onto/trajectory#TimeEntity"/>
        <rdfs:range rdf:resource="http://www.w3.org/2001/XMLSchema#dateTimeStamp"/>
        <rdfs:comment>A data property reused from the time ODP and describes when an event ends.</rdfs:comment>
    </owl:DatatypeProperty>
    


    <!-- 
    ///////////////////////////////////////////////////////////////////////////////////////
    //
    // Classes
    //
    ///////////////////////////////////////////////////////////////////////////////////////
     -->

    


    <!-- http://contextus.net/ontology/ontomedia/core/expression#Context -->

    <owl:Class rdf:about="http://contextus.net/ontology/ontomedia/core/expression#Context">
        <rdfs:subClassOf>
            <owl:Restriction>
                <owl:onProperty rdf:resource="http://www.kracr.iiitd.edu.in/ontology/apple/describesEvent"/>
                <owl:someValuesFrom rdf:resource="http://schema.org/Event"/>
            </owl:Restriction>
        </rdfs:subClassOf>
        <owl:disjointWith rdf:resource="http://www.kracr.iiitd.edu.in/ontology/apple/Ethics"/>
        <rdfs:comment xml:lang="en">This class represents the context in which an event or entity exists. (From OC Ontology: https://lov.linkeddata.es/dataset/lov/vocabs/oc).</rdfs:comment>
    </owl:Class>
    


    <!-- http://schema.mobivoc.org/Action -->

    <owl:Class rdf:about="http://schema.mobivoc.org/Action">
        <rdfs:subClassOf>
            <owl:Restriction>
                <owl:onProperty rdf:resource="http://www.kracr.iiitd.edu.in/ontology/apple/affects"/>
                <owl:someValuesFrom rdf:resource="http://www.kracr.iiitd.edu.in/ontology/apple/PassiveAgent"/>
            </owl:Restriction>
        </rdfs:subClassOf>
        <rdfs:subClassOf>
            <owl:Restriction>
                <owl:onProperty rdf:resource="http://www.kracr.iiitd.edu.in/ontology/apple/occursInEvent"/>
                <owl:someValuesFrom rdf:resource="http://schema.org/Event"/>
            </owl:Restriction>
        </rdfs:subClassOf>
        <rdfs:subClassOf>
            <owl:Restriction>
                <owl:onProperty rdf:resource="https://w3id.org/AIRO#hasConsequence"/>
                <owl:someValuesFrom rdf:resource="https://w3id.org/AIRO#Consequence"/>
            </owl:Restriction>
        </rdfs:subClassOf>
        <rdfs:comment xml:lang="en">Action that is done. (From schema: https://lov.linkeddata.es/dataset/lov/vocabs/mv)</rdfs:comment>
    </owl:Class>
    


    <!-- http://schema.org/Event -->

    <owl:Class rdf:about="http://schema.org/Event">
        <owl:equivalentClass rdf:resource="https://w3id.org/AIRO#Consequence"/>
        <rdfs:subClassOf>
            <owl:Restriction>
                <owl:onProperty rdf:resource="http://w3id.org/daselab/onto/trajectory#atPlace"/>
                <owl:someValuesFrom rdf:resource="http://w3id.org/daselab/onto/trajectory#Place"/>
            </owl:Restriction>
        </rdfs:subClassOf>
        <rdfs:subClassOf>
            <owl:Restriction>
                <owl:onProperty rdf:resource="http://w3id.org/daselab/onto/trajectory#atTime"/>
                <owl:someValuesFrom rdf:resource="http://w3id.org/daselab/onto/trajectory#TimeEntity"/>
            </owl:Restriction>
        </rdfs:subClassOf>
        <rdfs:subClassOf>
            <owl:Restriction>
                <owl:onProperty rdf:resource="http://www.kracr.iiitd.edu.in/ontology/apple/occursInDomain"/>
                <owl:someValuesFrom rdf:resource="https://w3id.org/AIRO#Domain"/>
            </owl:Restriction>
        </rdfs:subClassOf>
        <rdfs:subClassOf>
            <owl:Restriction>
                <owl:onProperty rdf:resource="http://www.ontologydesignpatterns.org/cp/owl/participation.owl#hasParticipant"/>
                <owl:someValuesFrom rdf:resource="http://xmlns.com/foaf/0.1/Agent"/>
            </owl:Restriction>
        </rdfs:subClassOf>
        <rdfs:subClassOf>
            <owl:Restriction>
                <owl:onProperty rdf:resource="http://www.ontologydesignpatterns.org/cp/owl/participation.owl#hasParticipant"/>
                <owl:someValuesFrom>
                    <owl:Class>
                        <owl:intersectionOf rdf:parseType="Collection">
                            <rdf:Description rdf:about="http://www.kracr.iiitd.edu.in/ontology/apple/ActiveAgent"/>
                            <rdf:Description rdf:about="http://www.kracr.iiitd.edu.in/ontology/apple/PassiveAgent"/>
                        </owl:intersectionOf>
                    </owl:Class>
                </owl:someValuesFrom>
            </owl:Restriction>
        </rdfs:subClassOf>
        <rdfs:comment xml:lang="en">An event happening at a certain time and location,&gt; property. Repeated events may be structured as separate Event objects. (From schema: https://lov.linkeddata.es/dataset/lov/vocabs/schema)</rdfs:comment>
        <rdfs:label>Event</rdfs:label>
    </owl:Class>
    


    <!-- http://w3id.org/daselab/onto/trajectory#Place -->

    <owl:Class rdf:about="http://w3id.org/daselab/onto/trajectory#Place">
        <rdfs:comment>This is the hook to other pattern/ontology that describes the notion of place, which is more general than just a location/geo-coordinate.</rdfs:comment>
        <rdfs:label>Place</rdfs:label>
    </owl:Class>
    


    <!-- http://w3id.org/daselab/onto/trajectory#TimeEntity -->

    <owl:Class rdf:about="http://w3id.org/daselab/onto/trajectory#TimeEntity">
        <rdfs:comment>The hook to class/pattern/ontology that models time, this class provides the temporal extent of the trajectory. One example of time model is the W3C Time Ontology.</rdfs:comment>
        <rdfs:label>Time</rdfs:label>
        <rdfs:seeAlso>http://www.w3.org/2006/time</rdfs:seeAlso>
    </owl:Class>
    


    <!-- http://www.kracr.iiitd.edu.in/ontology/apple#fromW3SWRL -->

    <owl:Class rdf:about="http://www.kracr.iiitd.edu.in/ontology/apple#fromW3SWRL">
        <rdfs:subClassOf rdf:resource="http://www.w3.org/2002/07/owl#Thing"/>
        <rdfs:comment>The elements used to apply SWRL Rules to the ApplE ontology. This class has been included to resolve important pitfalls.</rdfs:comment>
        <rdfs:label>fromW3SWRL</rdfs:label>
    </owl:Class>
    


    <!-- http://www.kracr.iiitd.edu.in/ontology/apple/AcademicDomain -->

    <owl:Class rdf:about="http://www.kracr.iiitd.edu.in/ontology/apple/AcademicDomain">
        <rdfs:subClassOf rdf:resource="http://www.kracr.iiitd.edu.in/ontology/apple/ProfessionalDomain"/>
        <rdfs:subClassOf>
            <owl:Restriction>
                <owl:onProperty rdf:resource="http://www.kracr.iiitd.edu.in/ontology/apple/adheresTo"/>
                <owl:someValuesFrom rdf:resource="http://www.kracr.iiitd.edu.in/ontology/apple/AcademicEthics"/>
            </owl:Restriction>
        </rdfs:subClassOf>
        <rdfs:subClassOf>
            <owl:Restriction>
                <owl:onProperty rdf:resource="http://www.kracr.iiitd.edu.in/ontology/apple/adheresTo"/>
                <owl:someValuesFrom rdf:resource="http://www.kracr.iiitd.edu.in/ontology/apple/ProfessionalEthics"/>
            </owl:Restriction>
        </rdfs:subClassOf>
        <rdfs:comment>The academic domain</rdfs:comment>
        <rdfs:comment>The domain that relates to the academic area which includes the impact of actions on students, teachers, administration staff, and the research community, along with the ethics of producing and disseminating research, and the conditions in which education is propagated.</rdfs:comment>
    </owl:Class>
    


    <!-- http://www.kracr.iiitd.edu.in/ontology/apple/AcademicEthics -->

    <owl:Class rdf:about="http://www.kracr.iiitd.edu.in/ontology/apple/AcademicEthics">
        <rdfs:subClassOf rdf:resource="http://www.kracr.iiitd.edu.in/ontology/apple/ProfessionalEthics"/>
        <rdfs:subClassOf>
            <owl:Restriction>
                <owl:onProperty rdf:resource="http://www.kracr.iiitd.edu.in/ontology/apple/appliesTo"/>
                <owl:someValuesFrom rdf:resource="http://www.kracr.iiitd.edu.in/ontology/apple/AcademicDomain"/>
            </owl:Restriction>
        </rdfs:subClassOf>
        <rdfs:subClassOf>
            <owl:Restriction>
                <owl:onProperty rdf:resource="http://www.kracr.iiitd.edu.in/ontology/apple/appliesTo"/>
                <owl:someValuesFrom rdf:resource="http://www.kracr.iiitd.edu.in/ontology/apple/ProfessionalDomain"/>
            </owl:Restriction>
        </rdfs:subClassOf>
        <owl:disjointWith rdf:resource="http://www.kracr.iiitd.edu.in/ontology/apple/BusinessEthics"/>
        <rdfs:comment>A field of applied ethics related to academic practices.</rdfs:comment>
    </owl:Class>
    


    <!-- http://www.kracr.iiitd.edu.in/ontology/apple/ActiveAgent -->

    <owl:Class rdf:about="http://www.kracr.iiitd.edu.in/ontology/apple/ActiveAgent">
        <rdfs:subClassOf rdf:resource="http://xmlns.com/foaf/0.1/Agent"/>
        <rdfs:subClassOf>
            <owl:Restriction>
                <owl:onProperty rdf:resource="http://www.kracr.iiitd.edu.in/ontology/apple/hasMoralIntention"/>
                <owl:someValuesFrom rdf:resource="http://www.kracr.iiitd.edu.in/ontology/apple/MoralIntention"/>
            </owl:Restriction>
        </rdfs:subClassOf>
        <rdfs:subClassOf>
            <owl:Restriction>
                <owl:onProperty rdf:resource="http://www.sensormeasurement.appspot.com/ont/transport/traffic#doesAction"/>
                <owl:someValuesFrom rdf:resource="http://schema.mobivoc.org/Action"/>
            </owl:Restriction>
        </rdfs:subClassOf>
        <rdfs:comment>An active agent is an agent that does the action in an event.</rdfs:comment>
        <rdfs:label>ActiveAgent</rdfs:label>
    </owl:Class>
    


    <!-- http://www.kracr.iiitd.edu.in/ontology/apple/AppliedEthics -->

    <owl:Class rdf:about="http://www.kracr.iiitd.edu.in/ontology/apple/AppliedEthics">
        <rdfs:subClassOf rdf:resource="http://www.kracr.iiitd.edu.in/ontology/apple/Ethics"/>
        <rdfs:subClassOf>
            <owl:Restriction>
                <owl:onProperty rdf:resource="http://www.kracr.iiitd.edu.in/ontology/apple/appliesPhilosophy"/>
                <owl:someValuesFrom rdf:resource="http://www.kracr.iiitd.edu.in/ontology/apple/AppliedEthicsPhilosophy"/>
            </owl:Restriction>
        </rdfs:subClassOf>
        <rdfs:subClassOf>
            <owl:Restriction>
                <owl:onProperty rdf:resource="http://www.kracr.iiitd.edu.in/ontology/apple/appliesTo"/>
                <owl:someValuesFrom rdf:resource="https://w3id.org/AIRO#Domain"/>
            </owl:Restriction>
        </rdfs:subClassOf>
        <rdfs:comment>Applied ethics is a sub-field of ethics, amongst the three major fields of the subject. It has to do with the application of ethical philosophies in various domains. 

Bioethics, for example, governs the applications of ethics in the medical domain. Similarly, professional ethics describes how ethical theories may be applied to the academic or corporate domains.</rdfs:comment>
    </owl:Class>
    


    <!-- http://www.kracr.iiitd.edu.in/ontology/apple/AppliedEthicsPhilosophy -->

    <owl:Class rdf:about="http://www.kracr.iiitd.edu.in/ontology/apple/AppliedEthicsPhilosophy">
        <rdfs:comment xml:lang="en">A philosophy that acts as a guiding principle to make ethical decisions pertaining to certain real-world domains.</rdfs:comment>
    </owl:Class>
    


    <!-- http://www.kracr.iiitd.edu.in/ontology/apple/BioethicsIssue -->

    <owl:Class rdf:about="http://www.kracr.iiitd.edu.in/ontology/apple/BioethicsIssue">
        <rdfs:subClassOf rdf:resource="http://www.kracr.iiitd.edu.in/ontology/apple/EthicalIssue"/>
        <rdfs:subClassOf>
            <owl:Restriction>
                <owl:onProperty rdf:resource="http://www.kracr.iiitd.edu.in/ontology/apple/resolvedBy"/>
                <owl:someValuesFrom rdf:resource="http://www.kracr.iiitd.edu.in/ontology/apple/BioethicsPhilosophy"/>
            </owl:Restriction>
        </rdfs:subClassOf>
        <rdfs:comment>A bioethics issue is an ethical issue that occurs in the medical domain.</rdfs:comment>
    </owl:Class>
    


    <!-- http://www.kracr.iiitd.edu.in/ontology/apple/BioethicsPhilosophy -->

    <owl:Class rdf:about="http://www.kracr.iiitd.edu.in/ontology/apple/BioethicsPhilosophy">
        <rdfs:subClassOf rdf:resource="http://www.kracr.iiitd.edu.in/ontology/apple/AppliedEthicsPhilosophy"/>
        <rdfs:comment xml:lang="en">A philosophy that acts as a guiding principle to make ethical decisions pertaining to bioethics in a real-world medical domain.</rdfs:comment>
    </owl:Class>
    


    <!-- http://www.kracr.iiitd.edu.in/ontology/apple/BusinessEthicalIssue -->

    <owl:Class rdf:about="http://www.kracr.iiitd.edu.in/ontology/apple/BusinessEthicalIssue">
        <rdfs:subClassOf rdf:resource="http://www.kracr.iiitd.edu.in/ontology/apple/EthicalIssue"/>
        <rdfs:subClassOf>
            <owl:Restriction>
                <owl:onProperty rdf:resource="http://www.kracr.iiitd.edu.in/ontology/apple/resolvedBy"/>
                <owl:someValuesFrom rdf:resource="http://www.kracr.iiitd.edu.in/ontology/apple/BusinessEthicsPhilosophy"/>
            </owl:Restriction>
        </rdfs:subClassOf>
        <rdfs:comment>A business ethical issue is an ethical issue that occurs in the professional domain.</rdfs:comment>
    </owl:Class>
    


    <!-- http://www.kracr.iiitd.edu.in/ontology/apple/BusinessEthics -->

    <owl:Class rdf:about="http://www.kracr.iiitd.edu.in/ontology/apple/BusinessEthics">
        <rdfs:subClassOf rdf:resource="http://www.kracr.iiitd.edu.in/ontology/apple/ProfessionalEthics"/>
        <rdfs:subClassOf>
            <owl:Restriction>
                <owl:onProperty rdf:resource="http://www.kracr.iiitd.edu.in/ontology/apple/appliesTo"/>
                <owl:someValuesFrom rdf:resource="http://www.kracr.iiitd.edu.in/ontology/apple/CorporateDomain"/>
            </owl:Restriction>
        </rdfs:subClassOf>
        <rdfs:subClassOf>
            <owl:Restriction>
                <owl:onProperty rdf:resource="http://www.kracr.iiitd.edu.in/ontology/apple/appliesTo"/>
                <owl:someValuesFrom rdf:resource="http://www.kracr.iiitd.edu.in/ontology/apple/ProfessionalDomain"/>
            </owl:Restriction>
        </rdfs:subClassOf>
        <rdfs:comment>A field of applied ethics related to the area of business and business practices.</rdfs:comment>
    </owl:Class>
    


    <!-- http://www.kracr.iiitd.edu.in/ontology/apple/BusinessEthicsPhilosophy -->

    <owl:Class rdf:about="http://www.kracr.iiitd.edu.in/ontology/apple/BusinessEthicsPhilosophy">
        <rdfs:subClassOf rdf:resource="http://www.kracr.iiitd.edu.in/ontology/apple/AppliedEthicsPhilosophy"/>
        <rdfs:comment xml:lang="en">A philosophy that acts as a guiding principle to make ethical decisions pertaining to business ethics in a real-world professional domain.</rdfs:comment>
    </owl:Class>
    


    <!-- http://www.kracr.iiitd.edu.in/ontology/apple/CharacteristicOfConsequence -->

    <owl:Class rdf:about="http://www.kracr.iiitd.edu.in/ontology/apple/CharacteristicOfConsequence">
        <rdfs:comment xml:lang="en">The characteristic of a consequence describes the impact of an action from the perspective of its duration, severity, and utility. The consequences of an action can have certain utilitarian and temporal aspects which may be defined using these characteristics.</rdfs:comment>
    </owl:Class>
    


    <!-- http://www.kracr.iiitd.edu.in/ontology/apple/Consequentialism -->

    <owl:Class rdf:about="http://www.kracr.iiitd.edu.in/ontology/apple/Consequentialism">
        <rdfs:subClassOf rdf:resource="http://www.kracr.iiitd.edu.in/ontology/apple/NormativeEthics"/>
        <rdfs:subClassOf>
            <owl:Restriction>
                <owl:onProperty rdf:resource="http://www.kracr.iiitd.edu.in/ontology/apple/associatedWith"/>
                <owl:someValuesFrom rdf:resource="https://w3id.org/AIRO#Consequence"/>
            </owl:Restriction>
        </rdfs:subClassOf>
        <rdfs:comment xml:lang="en">Consequentialism is an ethical theory that judges whether or not something is right by what its consequences are. For instance, most people would agree that lying is wrong. But if telling a lie would help save a person&apos;s life, consequentialism says it&apos;s the right thing to do.</rdfs:comment>
    </owl:Class>
    


    <!-- http://www.kracr.iiitd.edu.in/ontology/apple/ConsumerCentricBusinessEthicalIssue -->

    <owl:Class rdf:about="http://www.kracr.iiitd.edu.in/ontology/apple/ConsumerCentricBusinessEthicalIssue">
        <rdfs:subClassOf rdf:resource="http://www.kracr.iiitd.edu.in/ontology/apple/BusinessEthicalIssue"/>
        <rdfs:comment>A consumer-centric ethical issue is a business ethical issue that discusses the consequences of an action on one or more consumer(s).</rdfs:comment>
    </owl:Class>
    


    <!-- http://www.kracr.iiitd.edu.in/ontology/apple/CorporateDomain -->

    <owl:Class rdf:about="http://www.kracr.iiitd.edu.in/ontology/apple/CorporateDomain">
        <rdfs:subClassOf rdf:resource="http://www.kracr.iiitd.edu.in/ontology/apple/ProfessionalDomain"/>
        <rdfs:subClassOf>
            <owl:Restriction>
                <owl:onProperty rdf:resource="http://www.kracr.iiitd.edu.in/ontology/apple/adheresTo"/>
                <owl:someValuesFrom rdf:resource="http://www.kracr.iiitd.edu.in/ontology/apple/BusinessEthics"/>
            </owl:Restriction>
        </rdfs:subClassOf>
        <rdfs:subClassOf>
            <owl:Restriction>
                <owl:onProperty rdf:resource="http://www.kracr.iiitd.edu.in/ontology/apple/adheresTo"/>
                <owl:someValuesFrom rdf:resource="http://www.kracr.iiitd.edu.in/ontology/apple/ProfessionalEthics"/>
            </owl:Restriction>
        </rdfs:subClassOf>
    </owl:Class>
    


    <!-- http://www.kracr.iiitd.edu.in/ontology/apple/Deontology -->

    <owl:Class rdf:about="http://www.kracr.iiitd.edu.in/ontology/apple/Deontology">
        <rdfs:subClassOf rdf:resource="http://www.kracr.iiitd.edu.in/ontology/apple/NormativeEthics"/>
        <rdfs:subClassOf>
            <owl:Restriction>
                <owl:onProperty rdf:resource="http://www.kracr.iiitd.edu.in/ontology/apple/associatedWith"/>
                <owl:someValuesFrom rdf:resource="http://www.kracr.iiitd.edu.in/ontology/apple/EthicalPrinciple"/>
            </owl:Restriction>
        </rdfs:subClassOf>
        <rdfs:comment>Deontology is a topic under normative ethics that takes from Kantianism and has to do with what is right and what is wrong. If an action is intrinsically wrong then the committing of such an action would also be wrong or unethical according to this ethical theory.</rdfs:comment>
    </owl:Class>
    


    <!-- http://www.kracr.iiitd.edu.in/ontology/apple/DurationOfConsequence -->

    <owl:Class rdf:about="http://www.kracr.iiitd.edu.in/ontology/apple/DurationOfConsequence">
        <rdfs:subClassOf rdf:resource="http://www.kracr.iiitd.edu.in/ontology/apple/CharacteristicOfConsequence"/>
        <rdfs:subClassOf>
            <owl:Restriction>
                <owl:onProperty rdf:resource="http://www.kracr.iiitd.edu.in/ontology/apple/hasScore"/>
                <owl:minCardinality rdf:datatype="http://www.w3.org/2001/XMLSchema#nonNegativeInteger">1</owl:minCardinality>
            </owl:Restriction>
        </rdfs:subClassOf>
        <rdfs:comment xml:lang="en">The duration of a consequence could be either short-term or long-term and this aspect plays a role in the morality of an action. From a consequentialist viewpoint, if an action leads to a bad consequence as well as a good consequence, a temporal assessment can give insight into whether it is morally right or wrong. If the action leads to a bad short-term consequence but a good long-term consequence then it may be an overall morally right action.</rdfs:comment>
    </owl:Class>
    


    <!-- http://www.kracr.iiitd.edu.in/ontology/apple/EnvironmentalDomain -->

    <owl:Class rdf:about="http://www.kracr.iiitd.edu.in/ontology/apple/EnvironmentalDomain">
        <rdfs:subClassOf rdf:resource="https://w3id.org/AIRO#Domain"/>
        <rdfs:subClassOf>
            <owl:Restriction>
                <owl:onProperty rdf:resource="http://www.kracr.iiitd.edu.in/ontology/apple/adheresTo"/>
                <owl:someValuesFrom rdf:resource="http://www.kracr.iiitd.edu.in/ontology/apple/EnvironmentalEthics"/>
            </owl:Restriction>
        </rdfs:subClassOf>
    </owl:Class>
    


    <!-- http://www.kracr.iiitd.edu.in/ontology/apple/EnvironmentalEthicalIssue -->

    <owl:Class rdf:about="http://www.kracr.iiitd.edu.in/ontology/apple/EnvironmentalEthicalIssue">
        <rdfs:subClassOf rdf:resource="http://www.kracr.iiitd.edu.in/ontology/apple/EthicalIssue"/>
        <rdfs:subClassOf>
            <owl:Restriction>
                <owl:onProperty rdf:resource="http://www.kracr.iiitd.edu.in/ontology/apple/resolvedBy"/>
                <owl:someValuesFrom rdf:resource="http://www.kracr.iiitd.edu.in/ontology/apple/EnvironmentalEthicsPhilosophy"/>
            </owl:Restriction>
        </rdfs:subClassOf>
        <rdfs:comment>An environmental ethical issue is an ethical issue that occurs in the environmental domain.</rdfs:comment>
    </owl:Class>
    


    <!-- http://www.kracr.iiitd.edu.in/ontology/apple/EnvironmentalEthics -->

    <owl:Class rdf:about="http://www.kracr.iiitd.edu.in/ontology/apple/EnvironmentalEthics">
        <rdfs:subClassOf rdf:resource="http://www.kracr.iiitd.edu.in/ontology/apple/AppliedEthics"/>
        <rdfs:subClassOf>
            <owl:Restriction>
                <owl:onProperty rdf:resource="http://www.kracr.iiitd.edu.in/ontology/apple/appliesTo"/>
                <owl:someValuesFrom rdf:resource="http://www.kracr.iiitd.edu.in/ontology/apple/EnvironmentalDomain"/>
            </owl:Restriction>
        </rdfs:subClassOf>
        <rdfs:comment>Environmental ethics is a sub-field of applied ethics that discusses the application of ethical theories in the environmental domain.</rdfs:comment>
    </owl:Class>
    


    <!-- http://www.kracr.iiitd.edu.in/ontology/apple/EnvironmentalEthicsPhilosophy -->

    <owl:Class rdf:about="http://www.kracr.iiitd.edu.in/ontology/apple/EnvironmentalEthicsPhilosophy">
        <rdfs:subClassOf rdf:resource="http://www.kracr.iiitd.edu.in/ontology/apple/AppliedEthicsPhilosophy"/>
        <rdfs:comment xml:lang="en">A philosophy that acts as a guiding principle to make ethical decisions pertaining to environmental ethics in a real-world environmental sciences domain.</rdfs:comment>
    </owl:Class>
    


    <!-- http://www.kracr.iiitd.edu.in/ontology/apple/EthicalIssue -->

    <owl:Class rdf:about="http://www.kracr.iiitd.edu.in/ontology/apple/EthicalIssue">
        <rdfs:subClassOf>
            <owl:Restriction>
                <owl:onProperty rdf:resource="http://www.kracr.iiitd.edu.in/ontology/apple/resolvedBy"/>
                <owl:someValuesFrom rdf:resource="http://www.kracr.iiitd.edu.in/ontology/apple/AppliedEthicsPhilosophy"/>
            </owl:Restriction>
        </rdfs:subClassOf>
        <rdfs:comment>An ethical issue arises when an action causes an impact on certain entities, that are capable of receiving the consequences, while violating some ethical principles. An extension of this is an ethical dilemma, in which more than one courses of actions lead to certain ethical issues, making it difficult to choose between the available actions.</rdfs:comment>
    </owl:Class>
    


    <!-- http://www.kracr.iiitd.edu.in/ontology/apple/EthicalPrinciple -->

    <owl:Class rdf:about="http://www.kracr.iiitd.edu.in/ontology/apple/EthicalPrinciple">
        <rdfs:subClassOf>
            <owl:Restriction>
                <owl:onProperty rdf:resource="http://www.kracr.iiitd.edu.in/ontology/apple#violatedByAction"/>
                <owl:someValuesFrom rdf:resource="http://schema.mobivoc.org/Action"/>
            </owl:Restriction>
        </rdfs:subClassOf>
        <rdfs:comment>An ethical principle is a concept that describes some virtue that must be upheld to preseve the morality of an action. 

For example, autonomy is an ethical principle which must be upheld so as to not violate some basic aspect of human rights. The violation of this would be unethical.</rdfs:comment>
    </owl:Class>
    


    <!-- http://www.kracr.iiitd.edu.in/ontology/apple/Ethics -->

    <owl:Class rdf:about="http://www.kracr.iiitd.edu.in/ontology/apple/Ethics">
        <rdfs:subClassOf rdf:resource="http://www.w3.org/2002/07/owl#Thing"/>
        <rdfs:comment>Ethics is a field of study in philosophy that describes the morality of an action in terms of its rightness, wrongness, goodness, and badness.</rdfs:comment>
    </owl:Class>
    


    <!-- http://www.kracr.iiitd.edu.in/ontology/apple/EthicsOfCare -->

    <owl:Class rdf:about="http://www.kracr.iiitd.edu.in/ontology/apple/EthicsOfCare">
        <rdfs:subClassOf rdf:resource="http://www.kracr.iiitd.edu.in/ontology/apple/AppliedEthics"/>
        <rdfs:comment>The ethics of care is a sub-field of applied ethics that discusses the application of ethical theories in the care domain. Although this may be considered a subfield of bioethics, it may be applied to domains other than medicine and is this considered separately. Care ethics promotes compassion, sympathy, and kindness, especially in the care of vulnerable agents.</rdfs:comment>
    </owl:Class>
    


    <!-- http://www.kracr.iiitd.edu.in/ontology/apple/LegalEthics -->

    <owl:Class rdf:about="http://www.kracr.iiitd.edu.in/ontology/apple/LegalEthics">
        <rdfs:subClassOf rdf:resource="http://www.kracr.iiitd.edu.in/ontology/apple/AppliedEthics"/>
        <rdfs:comment>A field of applied ethics related to the use and practice of law.</rdfs:comment>
    </owl:Class>
    


    <!-- http://www.kracr.iiitd.edu.in/ontology/apple/MediaEthics -->

    <owl:Class rdf:about="http://www.kracr.iiitd.edu.in/ontology/apple/MediaEthics">
        <rdfs:subClassOf rdf:resource="http://www.kracr.iiitd.edu.in/ontology/apple/AppliedEthics"/>
        <rdfs:comment>A field of applied ethics related to the various forms of dissipating media.</rdfs:comment>
    </owl:Class>
    


    <!-- http://www.kracr.iiitd.edu.in/ontology/apple/MedicalDomain -->

    <owl:Class rdf:about="http://www.kracr.iiitd.edu.in/ontology/apple/MedicalDomain">
        <rdfs:subClassOf rdf:resource="https://w3id.org/AIRO#Domain"/>
        <rdfs:subClassOf>
            <owl:Restriction>
                <owl:onProperty rdf:resource="http://www.kracr.iiitd.edu.in/ontology/apple/adheresTo"/>
                <owl:someValuesFrom rdf:resource="https://w3id.org/skgo/modsci#Bioethics"/>
            </owl:Restriction>
        </rdfs:subClassOf>
    </owl:Class>
    


    <!-- http://www.kracr.iiitd.edu.in/ontology/apple/MetaEthics -->

    <owl:Class rdf:about="http://www.kracr.iiitd.edu.in/ontology/apple/MetaEthics">
        <rdfs:subClassOf rdf:resource="http://www.kracr.iiitd.edu.in/ontology/apple/Ethics"/>
        <rdfs:comment xml:lang="en">Metaethics is a branch of analytic philosophy that explores the status, foundations, and scope of moral values, properties, and words. Whereas the fields of applied ethics and normative theory focus on what is moral, metaethics focuses on what morality itself is. (From the Internet Encyclopedia of Philosophy)</rdfs:comment>
    </owl:Class>
    


    <!-- http://www.kracr.iiitd.edu.in/ontology/apple/MoralIntention -->

    <owl:Class rdf:about="http://www.kracr.iiitd.edu.in/ontology/apple/MoralIntention">
        <rdfs:comment xml:lang="en">Moral Intention is defined as the ability to prioritise moral values over other values and hence requires that the desired outcome is bound by moral values. 

(From A. C. Ping, Strategic Ethical Consultancy).

Moral intent is the desire to act ethically when facing a decision and overcome the rationalization to not be ethical “this time.” Even if a person sees the ethical aspects of a decision and has the philosophical tools to make the right choice, he or she still needs to want to do the right thing. If a person has no moral intent, then moral awareness and moral decision making are useless.

(From BEING YOUR BEST SELF, PART 3: MORAL INTENT, Ethics Unwrapped.)</rdfs:comment>
        <rdfs:label>MoralIntention</rdfs:label>
    </owl:Class>
    


    <!-- http://www.kracr.iiitd.edu.in/ontology/apple/MorallyGreyAction -->

    <owl:Class rdf:about="http://www.kracr.iiitd.edu.in/ontology/apple/MorallyGreyAction">
        <rdfs:subClassOf rdf:resource="http://schema.mobivoc.org/Action"/>
        <rdfs:subClassOf>
            <owl:Restriction>
                <owl:onProperty rdf:resource="http://www.kracr.iiitd.edu.in/ontology/apple/upholdsEthicalPrinciple"/>
                <owl:someValuesFrom rdf:resource="http://www.kracr.iiitd.edu.in/ontology/apple/EthicalPrinciple"/>
            </owl:Restriction>
        </rdfs:subClassOf>
        <rdfs:subClassOf>
            <owl:Restriction>
                <owl:onProperty rdf:resource="http://www.kracr.iiitd.edu.in/ontology/apple/violatesEthicalPrinciple"/>
                <owl:someValuesFrom rdf:resource="http://www.kracr.iiitd.edu.in/ontology/apple/EthicalPrinciple"/>
            </owl:Restriction>
        </rdfs:subClassOf>
        <rdfs:comment>An action that has some benefits and losses to the extent that it is indiscernible as to which is the better course of action is considered a morally grey action. It has equally good and bad moral value in terms of consequence, principle, and intention.</rdfs:comment>
    </owl:Class>
    


    <!-- http://www.kracr.iiitd.edu.in/ontology/apple/MorallyRightAction -->

    <owl:Class rdf:about="http://www.kracr.iiitd.edu.in/ontology/apple/MorallyRightAction">
        <rdfs:subClassOf rdf:resource="http://schema.mobivoc.org/Action"/>
        <rdfs:subClassOf>
            <owl:Restriction>
                <owl:onProperty rdf:resource="http://www.kracr.iiitd.edu.in/ontology/apple/upholdsEthicalPrinciple"/>
                <owl:someValuesFrom rdf:resource="http://www.kracr.iiitd.edu.in/ontology/apple/EthicalPrinciple"/>
            </owl:Restriction>
        </rdfs:subClassOf>
        <rdfs:comment>An action that is considered to be an ideal or correct course of action in a particular situation or event is a morally right action.</rdfs:comment>
    </owl:Class>
    


    <!-- http://www.kracr.iiitd.edu.in/ontology/apple/MorallyWrongAction -->

    <owl:Class rdf:about="http://www.kracr.iiitd.edu.in/ontology/apple/MorallyWrongAction">
        <rdfs:subClassOf rdf:resource="http://schema.mobivoc.org/Action"/>
        <rdfs:subClassOf>
            <owl:Restriction>
                <owl:onProperty rdf:resource="http://www.kracr.iiitd.edu.in/ontology/apple/violatesEthicalPrinciple"/>
                <owl:someValuesFrom rdf:resource="http://www.kracr.iiitd.edu.in/ontology/apple/EthicalPrinciple"/>
            </owl:Restriction>
        </rdfs:subClassOf>
        <rdfs:comment>An action that is considered to be a not ideal or wrong course of action in a particular situation or event is a morally wrong action.</rdfs:comment>
    </owl:Class>
    


    <!-- http://www.kracr.iiitd.edu.in/ontology/apple/NormativeEthics -->

    <owl:Class rdf:about="http://www.kracr.iiitd.edu.in/ontology/apple/NormativeEthics">
        <rdfs:subClassOf rdf:resource="http://www.kracr.iiitd.edu.in/ontology/apple/Ethics"/>
        <rdfs:comment>Normative ethics has to do with the foundational aspects of ethics which require the basic application of ethics in various domains.</rdfs:comment>
    </owl:Class>
    


    <!-- http://www.kracr.iiitd.edu.in/ontology/apple/PassiveAgent -->

    <owl:Class rdf:about="http://www.kracr.iiitd.edu.in/ontology/apple/PassiveAgent">
        <rdfs:subClassOf rdf:resource="http://xmlns.com/foaf/0.1/Agent"/>
        <rdfs:comment>A Passive agent is an agent that may be involved in an event and is directly affected by the action of the active agent.</rdfs:comment>
        <rdfs:label>PassiveAgent</rdfs:label>
    </owl:Class>
    


    <!-- http://www.kracr.iiitd.edu.in/ontology/apple/PoliticalEthics -->

    <owl:Class rdf:about="http://www.kracr.iiitd.edu.in/ontology/apple/PoliticalEthics">
        <rdfs:subClassOf rdf:resource="http://www.kracr.iiitd.edu.in/ontology/apple/AppliedEthics"/>
        <rdfs:comment>A field of applied ethics related to the area of politics and various political practices.</rdfs:comment>
    </owl:Class>
    


    <!-- http://www.kracr.iiitd.edu.in/ontology/apple/ProfessionalDomain -->

    <owl:Class rdf:about="http://www.kracr.iiitd.edu.in/ontology/apple/ProfessionalDomain">
        <rdfs:subClassOf rdf:resource="https://w3id.org/AIRO#Domain"/>
        <rdfs:comment>A professional domain involves aspects with relation to the workspace. The professional domain is, again, vast and includes offices, colleges, government, fieldwork, etc. However, it may be broadly categorized into the academic and corporate domains. It involves the ethics of employers towards their employees and vice versa, and how companies and institutions deal with the various stakeholders associated with their establishments.</rdfs:comment>
    </owl:Class>
    


    <!-- http://www.kracr.iiitd.edu.in/ontology/apple/ProfessionalEthics -->

    <owl:Class rdf:about="http://www.kracr.iiitd.edu.in/ontology/apple/ProfessionalEthics">
        <rdfs:subClassOf rdf:resource="http://www.kracr.iiitd.edu.in/ontology/apple/AppliedEthics"/>
        <rdfs:comment>A field of applied ethics related to the workplace. This may include specific areas such as academics and business.</rdfs:comment>
    </owl:Class>
    


    <!-- http://www.kracr.iiitd.edu.in/ontology/apple/SeverityOfConsequence -->

    <owl:Class rdf:about="http://www.kracr.iiitd.edu.in/ontology/apple/SeverityOfConsequence">
        <rdfs:subClassOf rdf:resource="http://www.kracr.iiitd.edu.in/ontology/apple/CharacteristicOfConsequence"/>
        <rdfs:subClassOf>
            <owl:Restriction>
                <owl:onProperty rdf:resource="http://www.kracr.iiitd.edu.in/ontology/apple/hasScore"/>
                <owl:minCardinality rdf:datatype="http://www.w3.org/2001/XMLSchema#nonNegativeInteger">1</owl:minCardinality>
            </owl:Restriction>
        </rdfs:subClassOf>
        <rdfs:comment xml:lang="en">The severity of a consequence is an important aspect when judging an action on the basis of its consequence. It also helps to delineate between different consequences. Considering if there are two bad consequences, then an acceptable suggestion would be to proceed with the lesser evil.</rdfs:comment>
    </owl:Class>
    


    <!-- http://www.kracr.iiitd.edu.in/ontology/apple/SocietyCentricBusinessEthicalIssue -->

    <owl:Class rdf:about="http://www.kracr.iiitd.edu.in/ontology/apple/SocietyCentricBusinessEthicalIssue">
        <rdfs:subClassOf rdf:resource="http://www.kracr.iiitd.edu.in/ontology/apple/BusinessEthicalIssue"/>
        <rdfs:comment>A society-centric ethical issue is a business ethical issue that discusses the consequences of an action on the society.</rdfs:comment>
    </owl:Class>
    


    <!-- http://www.kracr.iiitd.edu.in/ontology/apple/TechnologicalEthics -->

    <owl:Class rdf:about="http://www.kracr.iiitd.edu.in/ontology/apple/TechnologicalEthics">
        <rdfs:subClassOf rdf:resource="http://www.kracr.iiitd.edu.in/ontology/apple/AppliedEthics"/>
        <rdfs:comment>A field of applied ethics related to the development and deployment of technology.</rdfs:comment>
    </owl:Class>
    


    <!-- http://www.kracr.iiitd.edu.in/ontology/apple/UtilityOfConsequence -->

    <owl:Class rdf:about="http://www.kracr.iiitd.edu.in/ontology/apple/UtilityOfConsequence">
        <rdfs:subClassOf rdf:resource="http://www.kracr.iiitd.edu.in/ontology/apple/CharacteristicOfConsequence"/>
        <rdfs:subClassOf>
            <owl:Restriction>
                <owl:onProperty rdf:resource="http://www.kracr.iiitd.edu.in/ontology/apple/hasScore"/>
                <owl:minCardinality rdf:datatype="http://www.w3.org/2001/XMLSchema#nonNegativeInteger">1</owl:minCardinality>
            </owl:Restriction>
        </rdfs:subClassOf>
        <rdfs:comment xml:lang="en">The utility of consequence describes the affect of the action from a good and bad perspective. It is also important to note that some consequences are neither good nor bad, they are neutral. A stricter view states that all actions have some good and/or bad consequences. In an action where no consequence has occured, the action itself was futile, due to which it was a waste of energy for the agent, thus a bad consequence.</rdfs:comment>
    </owl:Class>
    


    <!-- http://www.kracr.iiitd.edu.in/ontology/apple/VirtueEthics -->

    <owl:Class rdf:about="http://www.kracr.iiitd.edu.in/ontology/apple/VirtueEthics">
        <rdfs:subClassOf rdf:resource="http://www.kracr.iiitd.edu.in/ontology/apple/NormativeEthics"/>
        <rdfs:subClassOf>
            <owl:Restriction>
                <owl:onProperty rdf:resource="http://www.kracr.iiitd.edu.in/ontology/apple/associatedWith"/>
                <owl:someValuesFrom rdf:resource="http://www.kracr.iiitd.edu.in/ontology/apple/MoralIntention"/>
            </owl:Restriction>
        </rdfs:subClassOf>
        <rdfs:comment>Virtue ethics describes an ethical action to be one that is done by a virtuous agent. A virutous agent is one that possesses certain virtues such as honestly, reliability, responsibility, and trustworthiness. These virtues are considered to be generally acceptable and preferred in society.</rdfs:comment>
    </owl:Class>
    


    <!-- http://www.kracr.iiitd.edu.in/ontology/apple/WorkerCentricBusinessEthicalIssue -->

    <owl:Class rdf:about="http://www.kracr.iiitd.edu.in/ontology/apple/WorkerCentricBusinessEthicalIssue">
        <rdfs:subClassOf rdf:resource="http://www.kracr.iiitd.edu.in/ontology/apple/BusinessEthicalIssue"/>
        <rdfs:comment>A worker-centric ethical issue is a business ethical issue that discusses the consequences of an action on one or more worker.</rdfs:comment>
        <rdfs:label>WorkerCentricBusinessEthicalIssue</rdfs:label>
    </owl:Class>
    


    <!-- http://www.ontologydesignpatterns.org/cp/owl/objectrole.owl#Role -->

    <owl:Class rdf:about="http://www.ontologydesignpatterns.org/cp/owl/objectrole.owl#Role">
        <rdfs:comment>A Concept that classifies an Object (in the case of the ApplE ontology, the role of an Agent).</rdfs:comment>
        <rdfs:label>Role</rdfs:label>
    </owl:Class>
    


    <!-- http://www.w3.org/2003/11/swrl#AtomList -->

    <owl:Class rdf:about="http://www.w3.org/2003/11/swrl#AtomList">
        <rdfs:subClassOf rdf:resource="http://www.kracr.iiitd.edu.in/ontology/apple#fromW3SWRL"/>
    </owl:Class>
    


    <!-- http://www.w3.org/2003/11/swrl#BuiltinAtom -->

    <owl:Class rdf:about="http://www.w3.org/2003/11/swrl#BuiltinAtom">
        <rdfs:subClassOf rdf:resource="http://www.kracr.iiitd.edu.in/ontology/apple#fromW3SWRL"/>
    </owl:Class>
    


    <!-- http://www.w3.org/2003/11/swrl#ClassAtom -->

    <owl:Class rdf:about="http://www.w3.org/2003/11/swrl#ClassAtom">
        <rdfs:subClassOf rdf:resource="http://www.kracr.iiitd.edu.in/ontology/apple#fromW3SWRL"/>
    </owl:Class>
    


    <!-- http://www.w3.org/2003/11/swrl#DatavaluedPropertyAtom -->

    <owl:Class rdf:about="http://www.w3.org/2003/11/swrl#DatavaluedPropertyAtom">
        <rdfs:subClassOf rdf:resource="http://www.kracr.iiitd.edu.in/ontology/apple#fromW3SWRL"/>
    </owl:Class>
    


    <!-- http://www.w3.org/2003/11/swrl#Imp -->

    <owl:Class rdf:about="http://www.w3.org/2003/11/swrl#Imp">
        <rdfs:subClassOf rdf:resource="http://www.kracr.iiitd.edu.in/ontology/apple#fromW3SWRL"/>
    </owl:Class>
    


    <!-- http://www.w3.org/2003/11/swrl#IndividualPropertyAtom -->

    <owl:Class rdf:about="http://www.w3.org/2003/11/swrl#IndividualPropertyAtom">
        <rdfs:subClassOf rdf:resource="http://www.kracr.iiitd.edu.in/ontology/apple#fromW3SWRL"/>
    </owl:Class>
    


    <!-- http://www.w3.org/2003/11/swrl#Variable -->

    <owl:Class rdf:about="http://www.w3.org/2003/11/swrl#Variable">
        <rdfs:subClassOf rdf:resource="http://www.kracr.iiitd.edu.in/ontology/apple#fromW3SWRL"/>
    </owl:Class>
    


    <!-- http://xmlns.com/foaf/0.1/Agent -->

    <owl:Class rdf:about="http://xmlns.com/foaf/0.1/Agent">
        <rdfs:subClassOf>
            <owl:Restriction>
                <owl:onProperty rdf:resource="http://www.ontologydesignpatterns.org/cp/owl/objectrole.owl#hasRole"/>
                <owl:someValuesFrom rdf:resource="http://www.ontologydesignpatterns.org/cp/owl/objectrole.owl#Role"/>
            </owl:Restriction>
        </rdfs:subClassOf>
        <rdfs:comment xml:lang="en">An agent (eg. person, group, software or physical artifact). (From foaf: https://lov.linkeddata.es/dataset/lov/vocabs/foaf)</rdfs:comment>
        <rdfs:label>Agent</rdfs:label>
    </owl:Class>
    


    <!-- https://w3id.org/AIRO#Consequence -->

    <owl:Class rdf:about="https://w3id.org/AIRO#Consequence">
        <rdfs:subClassOf>
            <owl:Restriction>
                <owl:onProperty rdf:resource="http://www.kracr.iiitd.edu.in/ontology/apple/hasCharacteristicOfConsequence"/>
                <owl:minQualifiedCardinality rdf:datatype="http://www.w3.org/2001/XMLSchema#nonNegativeInteger">1</owl:minQualifiedCardinality>
                <owl:onClass rdf:resource="http://www.kracr.iiitd.edu.in/ontology/apple/DurationOfConsequence"/>
            </owl:Restriction>
        </rdfs:subClassOf>
        <rdfs:subClassOf>
            <owl:Restriction>
                <owl:onProperty rdf:resource="http://www.kracr.iiitd.edu.in/ontology/apple/hasCharacteristicOfConsequence"/>
                <owl:minQualifiedCardinality rdf:datatype="http://www.w3.org/2001/XMLSchema#nonNegativeInteger">1</owl:minQualifiedCardinality>
                <owl:onClass rdf:resource="http://www.kracr.iiitd.edu.in/ontology/apple/SeverityOfConsequence"/>
            </owl:Restriction>
        </rdfs:subClassOf>
        <rdfs:subClassOf>
            <owl:Restriction>
                <owl:onProperty rdf:resource="http://www.kracr.iiitd.edu.in/ontology/apple/hasCharacteristicOfConsequence"/>
                <owl:minQualifiedCardinality rdf:datatype="http://www.w3.org/2001/XMLSchema#nonNegativeInteger">1</owl:minQualifiedCardinality>
                <owl:onClass rdf:resource="http://www.kracr.iiitd.edu.in/ontology/apple/UtilityOfConsequence"/>
            </owl:Restriction>
        </rdfs:subClassOf>
        <rdfs:comment>The outcome of an action that has occured in an event by an agent. The consequences can be categorized based on temporal factors (short-term, long-term) and also on the basis of utility (risks, opportunities). These together can give a decision maker an understanding of the action and whether it is morally right, wrong, or grey. (Consequence IRI from: https://lov.linkeddata.es/dataset/lov/vocabs/airo)</rdfs:comment>
    </owl:Class>
    


    <!-- https://w3id.org/AIRO#Domain -->

    <owl:Class rdf:about="https://w3id.org/AIRO#Domain">
        <rdfs:subClassOf>
            <owl:Restriction>
                <owl:onProperty rdf:resource="http://www.kracr.iiitd.edu.in/ontology/apple/adheresTo"/>
                <owl:someValuesFrom rdf:resource="http://www.kracr.iiitd.edu.in/ontology/apple/AppliedEthics"/>
            </owl:Restriction>
        </rdfs:subClassOf>
        <rdfs:comment xml:lang="en">Represents the sector/domain the AI system is intended to be used in. (From AIRO: https://lov.linkeddata.es/dataset/lov/vocabs/airo)

Here, we use domain in a more general sense for our purposes.</rdfs:comment>
    </owl:Class>
    


    <!-- https://w3id.org/skgo/modsci#Bioethics -->

    <owl:Class rdf:about="https://w3id.org/skgo/modsci#Bioethics">
        <rdfs:subClassOf rdf:resource="http://www.kracr.iiitd.edu.in/ontology/apple/AppliedEthics"/>
        <rdfs:subClassOf>
            <owl:Restriction>
                <owl:onProperty rdf:resource="http://www.kracr.iiitd.edu.in/ontology/apple/appliesTo"/>
                <owl:someValuesFrom rdf:resource="http://www.kracr.iiitd.edu.in/ontology/apple/MedicalDomain"/>
            </owl:Restriction>
        </rdfs:subClassOf>
        <rdfs:comment>Bioethics is a sub-field of applied ethics that discusses the application of ethical theories in the medical domain.</rdfs:comment>
    </owl:Class>
    


    <!-- 
    ///////////////////////////////////////////////////////////////////////////////////////
    //
    // Individuals
    //
    ///////////////////////////////////////////////////////////////////////////////////////
     -->

    


    <!-- http://www.kracr.iiitd.edu.in/ontology/apple#Bioethics -->

    <owl:NamedIndividual rdf:about="http://www.kracr.iiitd.edu.in/ontology/apple#Bioethics">
        <rdf:type rdf:resource="http://www.kracr.iiitd.edu.in/ontology/apple/Ethics"/>
        <rdf:type rdf:resource="https://w3id.org/skgo/modsci#Bioethics"/>
        <apple:appliesPhilosophy rdf:resource="http://www.kracr.iiitd.edu.in/ontology/apple/Principlism"/>
        <rdfs:comment>The study of ethical, social, and legal issues that arise in biomedicine and biomedical research</rdfs:comment>
    </owl:NamedIndividual>
    


    <!-- http://www.kracr.iiitd.edu.in/ontology/apple#BioethicsEventContext -->

    <owl:NamedIndividual rdf:about="http://www.kracr.iiitd.edu.in/ontology/apple#BioethicsEventContext">
        <rdf:type rdf:resource="http://contextus.net/ontology/ontomedia/core/expression#Context"/>
        <apple:describesEvent rdf:resource="http://www.kracr.iiitd.edu.in/ontology/apple#PrescriptionOfAddictiveDrug"/>
        <rdfs:comment>The context in which an event occurs in the medical domain.</rdfs:comment>
    </owl:NamedIndividual>
    


    <!-- http://www.kracr.iiitd.edu.in/ontology/apple#Clinic -->

    <owl:NamedIndividual rdf:about="http://www.kracr.iiitd.edu.in/ontology/apple#Clinic">
        <rdf:type rdf:resource="http://w3id.org/daselab/onto/trajectory#Place"/>
        <rdfs:comment>A space where outpatients recieve treatment or are referred to hospitals.</rdfs:comment>
    </owl:NamedIndividual>
    


    <!-- http://www.kracr.iiitd.edu.in/ontology/apple#Doctor -->

    <owl:NamedIndividual rdf:about="http://www.kracr.iiitd.edu.in/ontology/apple#Doctor">
        <rdf:type rdf:resource="http://www.kracr.iiitd.edu.in/ontology/apple/ActiveAgent"/>
        <apple:hasMoralIntention rdf:resource="http://www.kracr.iiitd.edu.in/ontology/apple/GoodMoralIntention"/>
        <coparticipation:coparticipatesWith rdf:resource="http://www.kracr.iiitd.edu.in/ontology/apple#Patient"/>
        <objectrole:hasRole rdf:resource="http://www.kracr.iiitd.edu.in/ontology/apple#Doctor"/>
        <traffic:doesAction rdf:resource="http://www.kracr.iiitd.edu.in/ontology/apple#PrescribeOpioidPainkiller"/>
    </owl:NamedIndividual>
    


    <!-- http://www.kracr.iiitd.edu.in/ontology/apple#MedicalError -->

    <owl:NamedIndividual rdf:about="http://www.kracr.iiitd.edu.in/ontology/apple#MedicalError">
        <rdf:type rdf:resource="http://www.kracr.iiitd.edu.in/ontology/apple/BioethicsIssue"/>
        <apple:resolvedBy rdf:resource="http://www.kracr.iiitd.edu.in/ontology/apple/CommonMorality"/>
        <apple:resolvedBy rdf:resource="http://www.kracr.iiitd.edu.in/ontology/apple/Principlism"/>
    </owl:NamedIndividual>
    


    <!-- http://www.kracr.iiitd.edu.in/ontology/apple#OpioidUseDisorder -->

    <owl:NamedIndividual rdf:about="http://www.kracr.iiitd.edu.in/ontology/apple#OpioidUseDisorder">
        <rdf:type rdf:resource="https://w3id.org/AIRO#Consequence"/>
        <hasDurationOfConsequence rdf:resource="http://www.kracr.iiitd.edu.in/ontology/apple/LongTermConsequence"/>
        <hasSeverityOfConsequence rdf:resource="http://www.kracr.iiitd.edu.in/ontology/apple/SignificantConsequence"/>
        <hasUtilityOfConsequence rdf:resource="http://www.kracr.iiitd.edu.in/ontology/apple/BadConsequence"/>
        <apple:causesEthicalIssue rdf:resource="http://www.kracr.iiitd.edu.in/ontology/apple#MedicalError"/>
    </owl:NamedIndividual>
    


    <!-- http://www.kracr.iiitd.edu.in/ontology/apple#PainRelief -->

    <owl:NamedIndividual rdf:about="http://www.kracr.iiitd.edu.in/ontology/apple#PainRelief">
        <rdf:type rdf:resource="https://w3id.org/AIRO#Consequence"/>
        <hasSeverityOfConsequence rdf:resource="http://www.kracr.iiitd.edu.in/ontology/apple/MildConsequence"/>
        <apple:hasCharacteristicOfConsequence rdf:resource="http://www.kracr.iiitd.edu.in/ontology/apple/GoodConsequence"/>
        <apple:hasCharacteristicOfConsequence rdf:resource="http://www.kracr.iiitd.edu.in/ontology/apple/MildConsequence"/>
        <apple:hasCharacteristicOfConsequence rdf:resource="http://www.kracr.iiitd.edu.in/ontology/apple/ShortTermConsequence"/>
    </owl:NamedIndividual>
    


    <!-- http://www.kracr.iiitd.edu.in/ontology/apple#Patient -->

    <owl:NamedIndividual rdf:about="http://www.kracr.iiitd.edu.in/ontology/apple#Patient">
        <rdf:type rdf:resource="http://www.kracr.iiitd.edu.in/ontology/apple/PassiveAgent"/>
        <objectrole:hasRole rdf:resource="http://www.kracr.iiitd.edu.in/ontology/apple#Patient"/>
    </owl:NamedIndividual>
    


    <!-- http://www.kracr.iiitd.edu.in/ontology/apple#PrescribeOpioidPainkiller -->

    <owl:NamedIndividual rdf:about="http://www.kracr.iiitd.edu.in/ontology/apple#PrescribeOpioidPainkiller">
        <rdf:type rdf:resource="http://schema.mobivoc.org/Action"/>
        <apple:upholdsEthicalPrinciple rdf:resource="http://www.kracr.iiitd.edu.in/ontology/apple/Beneficence"/>
        <apple:violatesEthicalPrinciple rdf:resource="http://www.kracr.iiitd.edu.in/ontology/apple/Nonmaleficence"/>
        <apple:violatesEthicalPrinciple rdf:resource="http://www.kracr.iiitd.edu.in/ontology/apple/Responsibility"/>
        <AIRO:hasConsequence rdf:resource="http://www.kracr.iiitd.edu.in/ontology/apple#OpioidUseDisorder"/>
        <AIRO:hasConsequence rdf:resource="http://www.kracr.iiitd.edu.in/ontology/apple#PainRelief"/>
        <rdfs:comment>The action by the doctor to prescribe an opioid painkiller.</rdfs:comment>
    </owl:NamedIndividual>
    


    <!-- http://www.kracr.iiitd.edu.in/ontology/apple#PrescriptionOfAddictiveDrug -->

    <owl:NamedIndividual rdf:about="http://www.kracr.iiitd.edu.in/ontology/apple#PrescriptionOfAddictiveDrug">
        <rdf:type rdf:resource="http://schema.org/Event"/>
        <event:hasInformationObject rdf:resource="http://www.kracr.iiitd.edu.in/ontology/apple#PrescribeOpioidPainkiller"/>
        <trajectory:atPlace rdf:resource="http://www.kracr.iiitd.edu.in/ontology/apple#Clinic"/>
        <trajectory:atTime rdf:resource="http://www.kracr.iiitd.edu.in/ontology/apple#1996"/>
        <apple:occursInDomain rdf:resource="http://www.kracr.iiitd.edu.in/ontology/apple/MedicalDomain"/>
        <participation:hasParticipant rdf:resource="http://www.kracr.iiitd.edu.in/ontology/apple#Doctor"/>
        <participation:hasParticipant rdf:resource="http://www.kracr.iiitd.edu.in/ontology/apple#Patient"/>
    </owl:NamedIndividual>
    


    <!-- http://www.kracr.iiitd.edu.in/ontology/apple#1996 -->

    <owl:NamedIndividual rdf:about="http://www.kracr.iiitd.edu.in/ontology/apple#1996">
        <rdf:type rdf:resource="http://w3id.org/daselab/onto/trajectory#TimeEntity"/>
        <time:hasBeginning rdf:datatype="http://www.w3.org/2001/XMLSchema#dateTime">1996-01-01T13:20:00Z</time:hasBeginning>
        <rdfs:comment>The year 1996.</rdfs:comment>
    </owl:NamedIndividual>
    


    <!-- http://www.kracr.iiitd.edu.in/ontology/apple/Abortion -->

    <owl:NamedIndividual rdf:about="http://www.kracr.iiitd.edu.in/ontology/apple/Abortion">
        <rdf:type rdf:resource="http://www.kracr.iiitd.edu.in/ontology/apple/BioethicsIssue"/>
        <rdfs:comment>Abortion is the process of deliberately ending a pregnancy.</rdfs:comment>
    </owl:NamedIndividual>
    


    <!-- http://www.kracr.iiitd.edu.in/ontology/apple/Animism -->

    <owl:NamedIndividual rdf:about="http://www.kracr.iiitd.edu.in/ontology/apple/Animism">
        <rdf:type rdf:resource="http://www.kracr.iiitd.edu.in/ontology/apple/EnvironmentalEthicsPhilosophy"/>
        <rdfs:comment>The attribution of a living soul to plants, inanimate objects, and natural phenomena.</rdfs:comment>
    </owl:NamedIndividual>
    


    <!-- http://www.kracr.iiitd.edu.in/ontology/apple/Anthropocentrism -->

    <owl:NamedIndividual rdf:about="http://www.kracr.iiitd.edu.in/ontology/apple/Anthropocentrism">
        <rdf:type rdf:resource="http://www.kracr.iiitd.edu.in/ontology/apple/EnvironmentalEthicsPhilosophy"/>
        <rdfs:comment>The ethical belief that humans alone possess intrinsic value.</rdfs:comment>
    </owl:NamedIndividual>
    


    <!-- http://www.kracr.iiitd.edu.in/ontology/apple/Autonomy -->

    <owl:NamedIndividual rdf:about="http://www.kracr.iiitd.edu.in/ontology/apple/Autonomy">
        <rdf:type rdf:resource="http://www.kracr.iiitd.edu.in/ontology/apple/EthicalPrinciple"/>
        <apple:hasScore rdf:datatype="http://www.w3.org/2001/XMLSchema#int">1</apple:hasScore>
        <rdfs:comment>In Kantian moral philosophy, the capacity of an agent to act in accordance with objective morality rather than under the influence of desires.</rdfs:comment>
    </owl:NamedIndividual>
    


    <!-- http://www.kracr.iiitd.edu.in/ontology/apple/BadConsequence -->

    <owl:NamedIndividual rdf:about="http://www.kracr.iiitd.edu.in/ontology/apple/BadConsequence">
        <rdf:type rdf:resource="http://www.kracr.iiitd.edu.in/ontology/apple/UtilityOfConsequence"/>
        <apple:hasScore rdf:datatype="http://www.w3.org/2001/XMLSchema#int">-1</apple:hasScore>
        <rdfs:comment>A consequence that has a negative moral value in accordance with its utility, principle, and moral intention.</rdfs:comment>
    </owl:NamedIndividual>
    


    <!-- http://www.kracr.iiitd.edu.in/ontology/apple/BadMoralIntention -->

    <owl:NamedIndividual rdf:about="http://www.kracr.iiitd.edu.in/ontology/apple/BadMoralIntention">
        <rdf:type rdf:resource="http://www.kracr.iiitd.edu.in/ontology/apple/MoralIntention"/>
        <apple:hasScore rdf:datatype="http://www.w3.org/2001/XMLSchema#int">-2</apple:hasScore>
        <rdfs:comment>A premeditated intention to cause harm or loss to another agent.</rdfs:comment>
    </owl:NamedIndividual>
    


    <!-- http://www.kracr.iiitd.edu.in/ontology/apple/Beneficence -->

    <owl:NamedIndividual rdf:about="http://www.kracr.iiitd.edu.in/ontology/apple/Beneficence">
        <rdf:type rdf:resource="http://www.kracr.iiitd.edu.in/ontology/apple/EthicalPrinciple"/>
        <apple:hasScore rdf:datatype="http://www.w3.org/2001/XMLSchema#int">1</apple:hasScore>
        <rdfs:comment>An act done with a strong connotation of doing good to others including moral obligation.</rdfs:comment>
    </owl:NamedIndividual>
    


    <!-- http://www.kracr.iiitd.edu.in/ontology/apple/Bioregionalism -->

    <owl:NamedIndividual rdf:about="http://www.kracr.iiitd.edu.in/ontology/apple/Bioregionalism">
        <rdf:type rdf:resource="http://www.kracr.iiitd.edu.in/ontology/apple/EnvironmentalEthicsPhilosophy"/>
        <rdfs:comment>Bioregionalism is a philosophy that suggests that political, cultural, and economic systems are more sustainable and just if they are organized around naturally defined areas called bioregions, similar to ecoregions.</rdfs:comment>
    </owl:NamedIndividual>
    


    <!-- http://www.kracr.iiitd.edu.in/ontology/apple/Casuistry -->

    <owl:NamedIndividual rdf:about="http://www.kracr.iiitd.edu.in/ontology/apple/Casuistry">
        <rdf:type rdf:resource="http://www.kracr.iiitd.edu.in/ontology/apple/BioethicsPhilosophy"/>
        <rdfs:comment>Casuistry is to do with discerning the ethics of an action based on several previous actions.</rdfs:comment>
    </owl:NamedIndividual>
    


    <!-- http://www.kracr.iiitd.edu.in/ontology/apple/ClimateChange -->

    <owl:NamedIndividual rdf:about="http://www.kracr.iiitd.edu.in/ontology/apple/ClimateChange">
        <rdf:type rdf:resource="http://www.kracr.iiitd.edu.in/ontology/apple/EnvironmentalEthicalIssue"/>
        <rdfs:comment>Climate change refers to long-term shifts in temperatures and weather patterns. (via UN)</rdfs:comment>
    </owl:NamedIndividual>
    


    <!-- http://www.kracr.iiitd.edu.in/ontology/apple/ClinicalResearch -->

    <owl:NamedIndividual rdf:about="http://www.kracr.iiitd.edu.in/ontology/apple/ClinicalResearch">
        <rdf:type rdf:resource="http://www.kracr.iiitd.edu.in/ontology/apple/BioethicsIssue"/>
        <rdfs:comment>The comprehensive study of the safety and effectiveness of the most promising advances in patient care.</rdfs:comment>
    </owl:NamedIndividual>
    


    <!-- http://www.kracr.iiitd.edu.in/ontology/apple/CommonMorality -->

    <owl:NamedIndividual rdf:about="http://www.kracr.iiitd.edu.in/ontology/apple/CommonMorality">
        <rdf:type rdf:resource="http://www.kracr.iiitd.edu.in/ontology/apple/BioethicsPhilosophy"/>
        <rdfs:comment>A moral system that everyone uses implicitly when making decisions and judgments.</rdfs:comment>
    </owl:NamedIndividual>
    


    <!-- http://www.kracr.iiitd.edu.in/ontology/apple/Compassion -->

    <owl:NamedIndividual rdf:about="http://www.kracr.iiitd.edu.in/ontology/apple/Compassion">
        <rdf:type rdf:resource="http://www.kracr.iiitd.edu.in/ontology/apple/EthicalPrinciple"/>
        <apple:hasScore rdf:datatype="http://www.w3.org/2001/XMLSchema#int">1</apple:hasScore>
        <rdfs:comment>Sympathetic pity and concern for the sufferings or misfortunes of others.</rdfs:comment>
    </owl:NamedIndividual>
    


    <!-- http://www.kracr.iiitd.edu.in/ontology/apple/Consent -->

    <owl:NamedIndividual rdf:about="http://www.kracr.iiitd.edu.in/ontology/apple/Consent">
        <rdf:type rdf:resource="http://www.kracr.iiitd.edu.in/ontology/apple/BioethicsIssue"/>
        <rdf:type rdf:resource="http://www.kracr.iiitd.edu.in/ontology/apple/ConsumerCentricBusinessEthicalIssue"/>
        <apple:resolvedBy rdf:resource="http://www.kracr.iiitd.edu.in/ontology/apple/StakeholderBalance"/>
        <rdfs:comment>Permission for something to happen or agreement to do something.</rdfs:comment>
    </owl:NamedIndividual>
    


    <!-- http://www.kracr.iiitd.edu.in/ontology/apple/CorporateDomain -->

    <owl:NamedIndividual rdf:about="http://www.kracr.iiitd.edu.in/ontology/apple/CorporateDomain">
        <rdf:type rdf:resource="https://w3id.org/AIRO#Domain"/>
    </owl:NamedIndividual>
    


    <!-- http://www.kracr.iiitd.edu.in/ontology/apple/CorporatePoliticalActivity -->

    <owl:NamedIndividual rdf:about="http://www.kracr.iiitd.edu.in/ontology/apple/CorporatePoliticalActivity">
        <rdf:type rdf:resource="http://www.kracr.iiitd.edu.in/ontology/apple/SocietyCentricBusinessEthicalIssue"/>
        <rdfs:comment>Corporate attempts to shape public policy</rdfs:comment>
    </owl:NamedIndividual>
    


    <!-- http://www.kracr.iiitd.edu.in/ontology/apple/CorporateSocialResponsibility -->

    <owl:NamedIndividual rdf:about="http://www.kracr.iiitd.edu.in/ontology/apple/CorporateSocialResponsibility">
        <rdf:type rdf:resource="http://www.kracr.iiitd.edu.in/ontology/apple/SocietyCentricBusinessEthicalIssue"/>
        <rdfs:comment>A theory that asserts that businesses should act in a manner that benefits the well-being of society and the environment.</rdfs:comment>
    </owl:NamedIndividual>
    


    <!-- http://www.kracr.iiitd.edu.in/ontology/apple/CullingFeralAnimals -->

    <owl:NamedIndividual rdf:about="http://www.kracr.iiitd.edu.in/ontology/apple/CullingFeralAnimals">
        <rdf:type rdf:resource="http://www.kracr.iiitd.edu.in/ontology/apple/EnvironmentalEthicalIssue"/>
        <rdfs:comment>The act of killing eliminated animals due to their feral nature and potential harm to their immediate ecosystem.</rdfs:comment>
    </owl:NamedIndividual>
    


    <!-- http://www.kracr.iiitd.edu.in/ontology/apple/CurbingOverpopulation -->

    <owl:NamedIndividual rdf:about="http://www.kracr.iiitd.edu.in/ontology/apple/CurbingOverpopulation">
        <rdf:type rdf:resource="http://www.kracr.iiitd.edu.in/ontology/apple/EnvironmentalEthicalIssue"/>
        <rdfs:comment>The steps that may be taken on a large scale to prevent a population explosion in highly populated regions.</rdfs:comment>
    </owl:NamedIndividual>
    


    <!-- http://www.kracr.iiitd.edu.in/ontology/apple/DeepEcology -->

    <owl:NamedIndividual rdf:about="http://www.kracr.iiitd.edu.in/ontology/apple/DeepEcology">
        <rdf:type rdf:resource="http://www.kracr.iiitd.edu.in/ontology/apple/EnvironmentalEthicsPhilosophy"/>
        <apple:resolves rdf:resource="http://www.kracr.iiitd.edu.in/ontology/apple/CullingFeralAnimals"/>
        <apple:resolves rdf:resource="http://www.kracr.iiitd.edu.in/ontology/apple/Deforestation"/>
        <rdfs:comment>The belief that nature has an inherent value.</rdfs:comment>
    </owl:NamedIndividual>
    


    <!-- http://www.kracr.iiitd.edu.in/ontology/apple/Deforestation -->

    <owl:NamedIndividual rdf:about="http://www.kracr.iiitd.edu.in/ontology/apple/Deforestation">
        <rdf:type rdf:resource="http://www.kracr.iiitd.edu.in/ontology/apple/EnvironmentalEthicalIssue"/>
        <rdfs:comment>The purposeful clearing of forested land.</rdfs:comment>
    </owl:NamedIndividual>
    


    <!-- http://www.kracr.iiitd.edu.in/ontology/apple/DeontologyForBusiness -->

    <owl:NamedIndividual rdf:about="http://www.kracr.iiitd.edu.in/ontology/apple/DeontologyForBusiness">
        <rdf:type rdf:resource="http://www.kracr.iiitd.edu.in/ontology/apple/BusinessEthicsPhilosophy"/>
        <rdf:type rdf:resource="http://www.kracr.iiitd.edu.in/ontology/apple/Ethics"/>
    </owl:NamedIndividual>
    


    <!-- http://www.kracr.iiitd.edu.in/ontology/apple/Dignity -->

    <owl:NamedIndividual rdf:about="http://www.kracr.iiitd.edu.in/ontology/apple/Dignity">
        <rdf:type rdf:resource="http://www.kracr.iiitd.edu.in/ontology/apple/EthicalPrinciple"/>
        <apple:hasScore rdf:datatype="http://www.w3.org/2001/XMLSchema#int">1</apple:hasScore>
    </owl:NamedIndividual>
    


    <!-- http://www.kracr.iiitd.edu.in/ontology/apple/DiscriminationInEmployment -->

    <owl:NamedIndividual rdf:about="http://www.kracr.iiitd.edu.in/ontology/apple/DiscriminationInEmployment">
        <rdf:type rdf:resource="http://www.kracr.iiitd.edu.in/ontology/apple/WorkerCentricBusinessEthicalIssue"/>
        <apple:resolvedBy rdf:resource="http://www.kracr.iiitd.edu.in/ontology/apple/StakeholderBalance"/>
    </owl:NamedIndividual>
    


    <!-- http://www.kracr.iiitd.edu.in/ontology/apple/Disenchantment -->

    <owl:NamedIndividual rdf:about="http://www.kracr.iiitd.edu.in/ontology/apple/Disenchantment">
        <rdf:type rdf:resource="http://www.kracr.iiitd.edu.in/ontology/apple/EnvironmentalEthicsPhilosophy"/>
    </owl:NamedIndividual>
    


    <!-- http://www.kracr.iiitd.edu.in/ontology/apple/DoNotResuscitate -->

    <owl:NamedIndividual rdf:about="http://www.kracr.iiitd.edu.in/ontology/apple/DoNotResuscitate">
        <rdf:type rdf:resource="http://www.kracr.iiitd.edu.in/ontology/apple/BioethicsIssue"/>
    </owl:NamedIndividual>
    


    <!-- http://www.kracr.iiitd.edu.in/ontology/apple/EnvironmentalDomain -->

    <owl:NamedIndividual rdf:about="http://www.kracr.iiitd.edu.in/ontology/apple/EnvironmentalDomain">
        <rdf:type rdf:resource="https://w3id.org/AIRO#Domain"/>
    </owl:NamedIndividual>
    


    <!-- http://www.kracr.iiitd.edu.in/ontology/apple/EpidemicContainment -->

    <owl:NamedIndividual rdf:about="http://www.kracr.iiitd.edu.in/ontology/apple/EpidemicContainment">
        <rdf:type rdf:resource="http://www.kracr.iiitd.edu.in/ontology/apple/EnvironmentalEthicalIssue"/>
    </owl:NamedIndividual>
    


    <!-- http://www.kracr.iiitd.edu.in/ontology/apple/Euthanasia -->

    <owl:NamedIndividual rdf:about="http://www.kracr.iiitd.edu.in/ontology/apple/Euthanasia">
        <rdf:type rdf:resource="http://www.kracr.iiitd.edu.in/ontology/apple/BioethicsIssue"/>
    </owl:NamedIndividual>
    


    <!-- http://www.kracr.iiitd.edu.in/ontology/apple/Fairness -->

    <owl:NamedIndividual rdf:about="http://www.kracr.iiitd.edu.in/ontology/apple/Fairness">
        <rdf:type rdf:resource="http://www.kracr.iiitd.edu.in/ontology/apple/EthicalPrinciple"/>
        <apple:hasScore rdf:datatype="http://www.w3.org/2001/XMLSchema#int">1</apple:hasScore>
    </owl:NamedIndividual>
    


    <!-- http://www.kracr.iiitd.edu.in/ontology/apple/Feminism -->

    <owl:NamedIndividual rdf:about="http://www.kracr.iiitd.edu.in/ontology/apple/Feminism">
        <rdf:type rdf:resource="http://www.kracr.iiitd.edu.in/ontology/apple/BioethicsPhilosophy"/>
        <rdf:type rdf:resource="http://www.kracr.iiitd.edu.in/ontology/apple/EnvironmentalEthicsPhilosophy"/>
    </owl:NamedIndividual>
    


    <!-- http://www.kracr.iiitd.edu.in/ontology/apple/FiringWithoutJustCause -->

    <owl:NamedIndividual rdf:about="http://www.kracr.iiitd.edu.in/ontology/apple/FiringWithoutJustCause">
        <rdf:type rdf:resource="http://www.kracr.iiitd.edu.in/ontology/apple/WorkerCentricBusinessEthicalIssue"/>
        <apple:resolvedBy rdf:resource="http://www.kracr.iiitd.edu.in/ontology/apple/StakeholderBalance"/>
    </owl:NamedIndividual>
    


    <!-- http://www.kracr.iiitd.edu.in/ontology/apple/GoodConsequence -->

    <owl:NamedIndividual rdf:about="http://www.kracr.iiitd.edu.in/ontology/apple/GoodConsequence">
        <rdf:type rdf:resource="http://www.kracr.iiitd.edu.in/ontology/apple/UtilityOfConsequence"/>
        <apple:hasScore rdf:datatype="http://www.w3.org/2001/XMLSchema#int">1</apple:hasScore>
    </owl:NamedIndividual>
    


    <!-- http://www.kracr.iiitd.edu.in/ontology/apple/GoodMoralIntention -->

    <owl:NamedIndividual rdf:about="http://www.kracr.iiitd.edu.in/ontology/apple/GoodMoralIntention">
        <rdf:type rdf:resource="http://www.kracr.iiitd.edu.in/ontology/apple/MoralIntention"/>
        <apple:hasScore rdf:datatype="http://www.w3.org/2001/XMLSchema#int">2</apple:hasScore>
    </owl:NamedIndividual>
    


    <!-- http://www.kracr.iiitd.edu.in/ontology/apple/HighTheory -->

    <owl:NamedIndividual rdf:about="http://www.kracr.iiitd.edu.in/ontology/apple/HighTheory">
        <rdf:type rdf:resource="http://www.kracr.iiitd.edu.in/ontology/apple/BioethicsPhilosophy"/>
    </owl:NamedIndividual>
    


    <!-- http://www.kracr.iiitd.edu.in/ontology/apple/Integrity -->

    <owl:NamedIndividual rdf:about="http://www.kracr.iiitd.edu.in/ontology/apple/Integrity">
        <rdf:type rdf:resource="http://www.kracr.iiitd.edu.in/ontology/apple/EthicalPrinciple"/>
        <apple:hasScore rdf:datatype="http://www.w3.org/2001/XMLSchema#int">1</apple:hasScore>
    </owl:NamedIndividual>
    


    <!-- http://www.kracr.iiitd.edu.in/ontology/apple/InternationalBusinessConcerns -->

    <owl:NamedIndividual rdf:about="http://www.kracr.iiitd.edu.in/ontology/apple/InternationalBusinessConcerns">
        <rdf:type rdf:resource="http://www.kracr.iiitd.edu.in/ontology/apple/SocietyCentricBusinessEthicalIssue"/>
        <apple:resolvedBy rdf:resource="http://www.kracr.iiitd.edu.in/ontology/apple/ShareholderPrimacy"/>
    </owl:NamedIndividual>
    


    <!-- http://www.kracr.iiitd.edu.in/ontology/apple/Justice -->

    <owl:NamedIndividual rdf:about="http://www.kracr.iiitd.edu.in/ontology/apple/Justice">
        <rdf:type rdf:resource="http://www.kracr.iiitd.edu.in/ontology/apple/EthicalPrinciple"/>
        <apple:hasScore rdf:datatype="http://www.w3.org/2001/XMLSchema#int">1</apple:hasScore>
    </owl:NamedIndividual>
    


    <!-- http://www.kracr.iiitd.edu.in/ontology/apple/LongTermConsequence -->

    <owl:NamedIndividual rdf:about="http://www.kracr.iiitd.edu.in/ontology/apple/LongTermConsequence">
        <rdf:type rdf:resource="http://www.kracr.iiitd.edu.in/ontology/apple/DurationOfConsequence"/>
        <apple:hasScore rdf:datatype="http://www.w3.org/2001/XMLSchema#int">2</apple:hasScore>
    </owl:NamedIndividual>
    


    <!-- http://www.kracr.iiitd.edu.in/ontology/apple/MarketFailuresApproach -->

    <owl:NamedIndividual rdf:about="http://www.kracr.iiitd.edu.in/ontology/apple/MarketFailuresApproach">
        <rdf:type rdf:resource="http://www.kracr.iiitd.edu.in/ontology/apple/BusinessEthicsPhilosophy"/>
    </owl:NamedIndividual>
    


    <!-- http://www.kracr.iiitd.edu.in/ontology/apple/MarketLimits -->

    <owl:NamedIndividual rdf:about="http://www.kracr.iiitd.edu.in/ontology/apple/MarketLimits">
        <rdf:type rdf:resource="http://www.kracr.iiitd.edu.in/ontology/apple/ConsumerCentricBusinessEthicalIssue"/>
    </owl:NamedIndividual>
    


    <!-- http://www.kracr.iiitd.edu.in/ontology/apple/MeaningfulWork -->

    <owl:NamedIndividual rdf:about="http://www.kracr.iiitd.edu.in/ontology/apple/MeaningfulWork">
        <rdf:type rdf:resource="http://www.kracr.iiitd.edu.in/ontology/apple/WorkerCentricBusinessEthicalIssue"/>
    </owl:NamedIndividual>
    


    <!-- http://www.kracr.iiitd.edu.in/ontology/apple/MedicalDomain -->

    <owl:NamedIndividual rdf:about="http://www.kracr.iiitd.edu.in/ontology/apple/MedicalDomain">
        <rdf:type rdf:resource="https://w3id.org/AIRO#Domain"/>
        <apple:adheresTo rdf:resource="http://www.kracr.iiitd.edu.in/ontology/apple#Bioethics"/>
    </owl:NamedIndividual>
    


    <!-- http://www.kracr.iiitd.edu.in/ontology/apple/MildConsequence -->

    <owl:NamedIndividual rdf:about="http://www.kracr.iiitd.edu.in/ontology/apple/MildConsequence">
        <rdf:type rdf:resource="http://www.kracr.iiitd.edu.in/ontology/apple/SeverityOfConsequence"/>
        <apple:hasScore rdf:datatype="http://www.w3.org/2001/XMLSchema#int">1</apple:hasScore>
        <rdfs:comment>A consequence that has a mild impact. The term &apos;mild&apos; may be subjective and comparative to other consequences. The choice of describing the severity of the consequence is upto the user.</rdfs:comment>
    </owl:NamedIndividual>
    


    <!-- http://www.kracr.iiitd.edu.in/ontology/apple/Misdiagnosis -->

    <owl:NamedIndividual rdf:about="http://www.kracr.iiitd.edu.in/ontology/apple/Misdiagnosis">
        <rdf:type rdf:resource="http://www.kracr.iiitd.edu.in/ontology/apple/BioethicsIssue"/>
    </owl:NamedIndividual>
    


    <!-- http://www.kracr.iiitd.edu.in/ontology/apple/ModerateConsequence -->

    <owl:NamedIndividual rdf:about="http://www.kracr.iiitd.edu.in/ontology/apple/ModerateConsequence">
        <rdf:type rdf:resource="http://www.kracr.iiitd.edu.in/ontology/apple/SeverityOfConsequence"/>
        <apple:hasScore rdf:datatype="http://www.w3.org/2001/XMLSchema#int">2</apple:hasScore>
        <rdfs:comment>A consequence that has a moderate impact. The term &apos;moderate&apos; may be subjective and comparative to other consequences. The choice of describing the severity of the consequence is upto the user.</rdfs:comment>
    </owl:NamedIndividual>
    


    <!-- http://www.kracr.iiitd.edu.in/ontology/apple/NarrativeEthics -->

    <owl:NamedIndividual rdf:about="http://www.kracr.iiitd.edu.in/ontology/apple/NarrativeEthics">
        <rdf:type rdf:resource="http://www.kracr.iiitd.edu.in/ontology/apple/BioethicsPhilosophy"/>
        <rdf:type rdf:resource="http://www.kracr.iiitd.edu.in/ontology/apple/Ethics"/>
    </owl:NamedIndividual>
    


    <!-- http://www.kracr.iiitd.edu.in/ontology/apple/NeutralConsequence -->

    <owl:NamedIndividual rdf:about="http://www.kracr.iiitd.edu.in/ontology/apple/NeutralConsequence">
        <rdf:type rdf:resource="http://www.kracr.iiitd.edu.in/ontology/apple/UtilityOfConsequence"/>
        <apple:hasScore rdf:datatype="http://www.w3.org/2001/XMLSchema#int">0</apple:hasScore>
    </owl:NamedIndividual>
    


    <!-- http://www.kracr.iiitd.edu.in/ontology/apple/NoMoralIntention -->

    <owl:NamedIndividual rdf:about="http://www.kracr.iiitd.edu.in/ontology/apple/NoMoralIntention">
        <rdf:type rdf:resource="http://www.kracr.iiitd.edu.in/ontology/apple/MoralIntention"/>
        <apple:hasScore rdf:datatype="http://www.w3.org/2001/XMLSchema#int">1</apple:hasScore>
    </owl:NamedIndividual>
    


    <!-- http://www.kracr.iiitd.edu.in/ontology/apple/Nonmaleficence -->

    <owl:NamedIndividual rdf:about="http://www.kracr.iiitd.edu.in/ontology/apple/Nonmaleficence">
        <rdf:type rdf:resource="http://www.kracr.iiitd.edu.in/ontology/apple/EthicalPrinciple"/>
        <apple:hasScore rdf:datatype="http://www.w3.org/2001/XMLSchema#int">1</apple:hasScore>
    </owl:NamedIndividual>
    


    <!-- http://www.kracr.iiitd.edu.in/ontology/apple/PandemicContainment -->

    <owl:NamedIndividual rdf:about="http://www.kracr.iiitd.edu.in/ontology/apple/PandemicContainment">
        <rdf:type rdf:resource="http://www.kracr.iiitd.edu.in/ontology/apple/EnvironmentalEthicalIssue"/>
    </owl:NamedIndividual>
    


    <!-- http://www.kracr.iiitd.edu.in/ontology/apple/PesticidesInAgriculture -->

    <owl:NamedIndividual rdf:about="http://www.kracr.iiitd.edu.in/ontology/apple/PesticidesInAgriculture">
        <rdf:type rdf:resource="http://www.kracr.iiitd.edu.in/ontology/apple/EnvironmentalEthicalIssue"/>
    </owl:NamedIndividual>
    


    <!-- http://www.kracr.iiitd.edu.in/ontology/apple/Pleasure -->

    <owl:NamedIndividual rdf:about="http://www.kracr.iiitd.edu.in/ontology/apple/Pleasure">
        <rdf:type rdf:resource="http://www.kracr.iiitd.edu.in/ontology/apple/EthicalPrinciple"/>
        <apple:hasScore rdf:datatype="http://www.w3.org/2001/XMLSchema#int">1</apple:hasScore>
    </owl:NamedIndividual>
    


    <!-- http://www.kracr.iiitd.edu.in/ontology/apple/PoliticalTheory -->

    <owl:NamedIndividual rdf:about="http://www.kracr.iiitd.edu.in/ontology/apple/PoliticalTheory">
        <rdf:type rdf:resource="http://www.kracr.iiitd.edu.in/ontology/apple/BusinessEthicsPhilosophy"/>
    </owl:NamedIndividual>
    


    <!-- http://www.kracr.iiitd.edu.in/ontology/apple/PriceDiscrimination -->

    <owl:NamedIndividual rdf:about="http://www.kracr.iiitd.edu.in/ontology/apple/PriceDiscrimination">
        <rdf:type rdf:resource="http://www.kracr.iiitd.edu.in/ontology/apple/ConsumerCentricBusinessEthicalIssue"/>
        <apple:resolvedBy rdf:resource="http://www.kracr.iiitd.edu.in/ontology/apple/StakeholderBalance"/>
    </owl:NamedIndividual>
    


    <!-- http://www.kracr.iiitd.edu.in/ontology/apple/PriceGouging -->

    <owl:NamedIndividual rdf:about="http://www.kracr.iiitd.edu.in/ontology/apple/PriceGouging">
        <rdf:type rdf:resource="http://www.kracr.iiitd.edu.in/ontology/apple/ConsumerCentricBusinessEthicalIssue"/>
    </owl:NamedIndividual>
    


    <!-- http://www.kracr.iiitd.edu.in/ontology/apple/Principlism -->

    <owl:NamedIndividual rdf:about="http://www.kracr.iiitd.edu.in/ontology/apple/Principlism">
        <rdf:type rdf:resource="http://www.kracr.iiitd.edu.in/ontology/apple/BioethicsPhilosophy"/>
    </owl:NamedIndividual>
    


    <!-- http://www.kracr.iiitd.edu.in/ontology/apple/Privacy -->

    <owl:NamedIndividual rdf:about="http://www.kracr.iiitd.edu.in/ontology/apple/Privacy">
        <rdf:type rdf:resource="http://www.kracr.iiitd.edu.in/ontology/apple/EthicalPrinciple"/>
        <apple:hasScore rdf:datatype="http://www.w3.org/2001/XMLSchema#int">1</apple:hasScore>
    </owl:NamedIndividual>
    


    <!-- http://www.kracr.iiitd.edu.in/ontology/apple/ProductSafety -->

    <owl:NamedIndividual rdf:about="http://www.kracr.iiitd.edu.in/ontology/apple/ProductSafety">
        <rdf:type rdf:resource="http://www.kracr.iiitd.edu.in/ontology/apple/ConsumerCentricBusinessEthicalIssue"/>
        <apple:resolvedBy rdf:resource="http://www.kracr.iiitd.edu.in/ontology/apple/StakeholderBalance"/>
    </owl:NamedIndividual>
    


    <!-- http://www.kracr.iiitd.edu.in/ontology/apple/ReflectiveEquilibrium -->

    <owl:NamedIndividual rdf:about="http://www.kracr.iiitd.edu.in/ontology/apple/ReflectiveEquilibrium">
        <rdf:type rdf:resource="http://www.kracr.iiitd.edu.in/ontology/apple/BioethicsPhilosophy"/>
    </owl:NamedIndividual>
    


    <!-- http://www.kracr.iiitd.edu.in/ontology/apple/RefusalToSell -->

    <owl:NamedIndividual rdf:about="http://www.kracr.iiitd.edu.in/ontology/apple/RefusalToSell">
        <rdf:type rdf:resource="http://www.kracr.iiitd.edu.in/ontology/apple/ConsumerCentricBusinessEthicalIssue"/>
    </owl:NamedIndividual>
    


    <!-- http://www.kracr.iiitd.edu.in/ontology/apple/ResourceAllocation -->

    <owl:NamedIndividual rdf:about="http://www.kracr.iiitd.edu.in/ontology/apple/ResourceAllocation">
        <rdf:type rdf:resource="http://www.kracr.iiitd.edu.in/ontology/apple/BioethicsIssue"/>
        <rdf:type rdf:resource="http://www.kracr.iiitd.edu.in/ontology/apple/EnvironmentalEthicalIssue"/>
    </owl:NamedIndividual>
    


    <!-- http://www.kracr.iiitd.edu.in/ontology/apple/ResourceExploitation -->

    <owl:NamedIndividual rdf:about="http://www.kracr.iiitd.edu.in/ontology/apple/ResourceExploitation">
        <rdf:type rdf:resource="http://www.kracr.iiitd.edu.in/ontology/apple/EnvironmentalEthicalIssue"/>
    </owl:NamedIndividual>
    


    <!-- http://www.kracr.iiitd.edu.in/ontology/apple/Responsibility -->

    <owl:NamedIndividual rdf:about="http://www.kracr.iiitd.edu.in/ontology/apple/Responsibility">
        <rdf:type rdf:resource="http://www.kracr.iiitd.edu.in/ontology/apple/EthicalPrinciple"/>
        <apple:hasScore rdf:datatype="http://www.w3.org/2001/XMLSchema#int">1</apple:hasScore>
    </owl:NamedIndividual>
    


    <!-- http://www.kracr.iiitd.edu.in/ontology/apple/ShareholderPrimacy -->

    <owl:NamedIndividual rdf:about="http://www.kracr.iiitd.edu.in/ontology/apple/ShareholderPrimacy">
        <rdf:type rdf:resource="http://www.kracr.iiitd.edu.in/ontology/apple/BusinessEthicsPhilosophy"/>
    </owl:NamedIndividual>
    


    <!-- http://www.kracr.iiitd.edu.in/ontology/apple/ShortTermConsequence -->

    <owl:NamedIndividual rdf:about="http://www.kracr.iiitd.edu.in/ontology/apple/ShortTermConsequence">
        <rdf:type rdf:resource="http://www.kracr.iiitd.edu.in/ontology/apple/DurationOfConsequence"/>
        <apple:hasScore rdf:datatype="http://www.w3.org/2001/XMLSchema#int">1</apple:hasScore>
    </owl:NamedIndividual>
    


    <!-- http://www.kracr.iiitd.edu.in/ontology/apple/SignificantConsequence -->

    <owl:NamedIndividual rdf:about="http://www.kracr.iiitd.edu.in/ontology/apple/SignificantConsequence">
        <rdf:type rdf:resource="http://www.kracr.iiitd.edu.in/ontology/apple/SeverityOfConsequence"/>
        <apple:hasScore rdf:datatype="http://www.w3.org/2001/XMLSchema#int">3</apple:hasScore>
        <rdfs:comment>A consequence that has a severe impact. The term &apos;severe&apos; may be subjective and comparative to other consequences. The choice of describing the severity of the consequence is upto the user.</rdfs:comment>
    </owl:NamedIndividual>
    


    <!-- http://www.kracr.iiitd.edu.in/ontology/apple/SocialEcology -->

    <owl:NamedIndividual rdf:about="http://www.kracr.iiitd.edu.in/ontology/apple/SocialEcology">
        <rdf:type rdf:resource="http://www.kracr.iiitd.edu.in/ontology/apple/EnvironmentalEthicsPhilosophy"/>
        <rdfs:comment>Social ecology studies relationships between people and their environment, often the interdependence of people, collectives and institutions.</rdfs:comment>
    </owl:NamedIndividual>
    


    <!-- http://www.kracr.iiitd.edu.in/ontology/apple/Solidarity -->

    <owl:NamedIndividual rdf:about="http://www.kracr.iiitd.edu.in/ontology/apple/Solidarity">
        <rdf:type rdf:resource="http://www.kracr.iiitd.edu.in/ontology/apple/EthicalPrinciple"/>
        <apple:hasScore rdf:datatype="http://www.w3.org/2001/XMLSchema#int">1</apple:hasScore>
        <rdfs:comment>Unity or agreement of feeling or action.</rdfs:comment>
    </owl:NamedIndividual>
    


    <!-- http://www.kracr.iiitd.edu.in/ontology/apple/StakeholderBalance -->

    <owl:NamedIndividual rdf:about="http://www.kracr.iiitd.edu.in/ontology/apple/StakeholderBalance">
        <rdf:type rdf:resource="http://www.kracr.iiitd.edu.in/ontology/apple/BusinessEthicsPhilosophy"/>
        <rdfs:comment>Stakeholder balance ensures that all individuals or groups with a vested interest in the company or the project have aligned interests and are compensated fairly without significant compromise from one party over another.</rdfs:comment>
    </owl:NamedIndividual>
    


    <!-- http://www.kracr.iiitd.edu.in/ontology/apple/Sustainability -->

    <owl:NamedIndividual rdf:about="http://www.kracr.iiitd.edu.in/ontology/apple/Sustainability">
        <rdf:type rdf:resource="http://www.kracr.iiitd.edu.in/ontology/apple/EnvironmentalEthicalIssue"/>
        <rdfs:comment>Sustainability is an environmental issue that has to do with reusing resources for energy generation and regular consumption in order to utilize them for longer.</rdfs:comment>
    </owl:NamedIndividual>
    


    <!-- http://www.kracr.iiitd.edu.in/ontology/apple/ToxicWorkEnvironment -->

    <owl:NamedIndividual rdf:about="http://www.kracr.iiitd.edu.in/ontology/apple/ToxicWorkEnvironment">
        <rdf:type rdf:resource="http://www.kracr.iiitd.edu.in/ontology/apple/WorkerCentricBusinessEthicalIssue"/>
        <rdfs:comment>A toxic work environment is one where negative, antagonistic, or bullying behavior is highly prominent at the workplace.</rdfs:comment>
    </owl:NamedIndividual>
    


    <!-- http://www.kracr.iiitd.edu.in/ontology/apple/Transparency -->

    <owl:NamedIndividual rdf:about="http://www.kracr.iiitd.edu.in/ontology/apple/Transparency">
        <rdf:type rdf:resource="http://www.kracr.iiitd.edu.in/ontology/apple/EthicalPrinciple"/>
        <apple:hasScore rdf:datatype="http://www.w3.org/2001/XMLSchema#int">1</apple:hasScore>
        <rdfs:comment>Transparency is a principle that has to do with a clarity of motives and procedure regarding a certain action.</rdfs:comment>
    </owl:NamedIndividual>
    


    <!-- http://www.kracr.iiitd.edu.in/ontology/apple/UnethicalAdvertising -->

    <owl:NamedIndividual rdf:about="http://www.kracr.iiitd.edu.in/ontology/apple/UnethicalAdvertising">
        <rdf:type rdf:resource="http://www.kracr.iiitd.edu.in/ontology/apple/ConsumerCentricBusinessEthicalIssue"/>
        <rdfs:comment>Unethical advertising practices advertise a product or product feature in a controversial way to persuade a customer to buy it. (via IGI Global)</rdfs:comment>
    </owl:NamedIndividual>
    


    <!-- http://www.kracr.iiitd.edu.in/ontology/apple/UnreasonableCompensation -->

    <owl:NamedIndividual rdf:about="http://www.kracr.iiitd.edu.in/ontology/apple/UnreasonableCompensation">
        <rdf:type rdf:resource="http://www.kracr.iiitd.edu.in/ontology/apple/WorkerCentricBusinessEthicalIssue"/>
        <apple:resolvedBy rdf:resource="http://www.kracr.iiitd.edu.in/ontology/apple/StakeholderBalance"/>
        <rdfs:comment>Unreasonable compensation is a level of compensation for owner-managers that does not meet the requirements for reasonable compensation. This may be either too low a compensation level or too high, depending upon the form of incorporation. (via Economic Research Institute)</rdfs:comment>
    </owl:NamedIndividual>
    


    <!-- http://www.kracr.iiitd.edu.in/ontology/apple/VirtueEthicsForBusiness -->

    <owl:NamedIndividual rdf:about="http://www.kracr.iiitd.edu.in/ontology/apple/VirtueEthicsForBusiness">
        <rdf:type rdf:resource="http://www.kracr.iiitd.edu.in/ontology/apple/BusinessEthicsPhilosophy"/>
        <rdfs:comment>Virtue ethics in business favors the demonstration of virtues such as honesty, diligence, responsibility, and compassion at the workplace.</rdfs:comment>
    </owl:NamedIndividual>
    


    <!-- http://www.kracr.iiitd.edu.in/ontology/apple/Whistleblowing -->

    <owl:NamedIndividual rdf:about="http://www.kracr.iiitd.edu.in/ontology/apple/Whistleblowing">
        <rdf:type rdf:resource="http://www.kracr.iiitd.edu.in/ontology/apple/WorkerCentricBusinessEthicalIssue"/>
        <rdfs:comment>Whistleblowing is the lawful disclosure of information a discloser reasonably believes evidences wrongdoing to an authorized recipient. (via DNI.gov)</rdfs:comment>
    </owl:NamedIndividual>
    


    <!-- 
    ///////////////////////////////////////////////////////////////////////////////////////
    //
    // Annotations
    //
    ///////////////////////////////////////////////////////////////////////////////////////
     -->

    <rdf:Description rdf:about="http://www.kracr.iiitd.edu.in/ontology/apple/CorporateDomain">
        <rdfs:comment>This domain has to do with the ethics of entities at the workplace and relates to the impact of actions on workers, consumers, stakeholders, shareholders, etc.</rdfs:comment>
    </rdf:Description>
    <rdf:Description rdf:about="http://www.kracr.iiitd.edu.in/ontology/apple/EnvironmentalDomain">
        <rdfs:comment>The domain of environmental sciences. It relates with the impact of actions on the environment.</rdfs:comment>
    </rdf:Description>
    <rdf:Description rdf:about="http://www.kracr.iiitd.edu.in/ontology/apple/MedicalDomain">
        <rdfs:comment>The domain of medical sciences. It relates with the impact of actions on patients, medical practitioners, medical institutions and establishments, the medical research areas and methods of research, etc.</rdfs:comment>
    </rdf:Description>
    


    <!-- 
    ///////////////////////////////////////////////////////////////////////////////////////
    //
    // General axioms
    //
    ///////////////////////////////////////////////////////////////////////////////////////
     -->

    <rdf:Description>
        <rdf:type rdf:resource="http://www.w3.org/2002/07/owl#AllDisjointClasses"/>
        <owl:members rdf:parseType="Collection">
            <rdf:Description rdf:about="http://www.kracr.iiitd.edu.in/ontology/apple/AppliedEthics"/>
            <rdf:Description rdf:about="http://www.kracr.iiitd.edu.in/ontology/apple/MetaEthics"/>
            <rdf:Description rdf:about="http://www.kracr.iiitd.edu.in/ontology/apple/NormativeEthics"/>
        </owl:members>
    </rdf:Description>
    <rdf:Description>
        <rdf:type rdf:resource="http://www.w3.org/2002/07/owl#AllDisjointClasses"/>
        <owl:members rdf:parseType="Collection">
            <rdf:Description rdf:about="http://www.kracr.iiitd.edu.in/ontology/apple/AppliedEthicsPhilosophy"/>
            <rdf:Description rdf:about="http://www.kracr.iiitd.edu.in/ontology/apple/EthicalIssue"/>
            <rdf:Description rdf:about="http://www.kracr.iiitd.edu.in/ontology/apple/EthicalPrinciple"/>
        </owl:members>
    </rdf:Description>
    <rdf:Description>
        <rdf:type rdf:resource="http://www.w3.org/2002/07/owl#AllDisjointClasses"/>
        <owl:members rdf:parseType="Collection">
            <rdf:Description rdf:about="http://www.kracr.iiitd.edu.in/ontology/apple/Consequentialism"/>
            <rdf:Description rdf:about="http://www.kracr.iiitd.edu.in/ontology/apple/Deontology"/>
            <rdf:Description rdf:about="http://www.kracr.iiitd.edu.in/ontology/apple/VirtueEthics"/>
        </owl:members>
    </rdf:Description>
    <rdf:Description>
        <rdf:type rdf:resource="http://www.w3.org/2002/07/owl#AllDisjointClasses"/>
        <owl:members rdf:parseType="Collection">
            <rdf:Description rdf:about="http://www.kracr.iiitd.edu.in/ontology/apple/DurationOfConsequence"/>
            <rdf:Description rdf:about="http://www.kracr.iiitd.edu.in/ontology/apple/SeverityOfConsequence"/>
            <rdf:Description rdf:about="http://www.kracr.iiitd.edu.in/ontology/apple/UtilityOfConsequence"/>
        </owl:members>
    </rdf:Description>
    


    <!-- 
    ///////////////////////////////////////////////////////////////////////////////////////
    //
    // Rules
    //
    ///////////////////////////////////////////////////////////////////////////////////////
     -->

    <rdf:Description rdf:about="urn:swrl:var#ag">
        <rdf:type rdf:resource="http://www.w3.org/2003/11/swrl#Variable"/>
    </rdf:Description>
    <rdf:Description rdf:about="urn:swrl:var#a">
        <rdf:type rdf:resource="http://www.w3.org/2003/11/swrl#Variable"/>
    </rdf:Description>
    <rdf:Description rdf:about="urn:swrl:var#c">
        <rdf:type rdf:resource="http://www.w3.org/2003/11/swrl#Variable"/>
    </rdf:Description>
    <rdf:Description rdf:about="urn:swrl:var#soc">
        <rdf:type rdf:resource="http://www.w3.org/2003/11/swrl#Variable"/>
    </rdf:Description>
    <rdf:Description rdf:about="urn:swrl:var#uoc">
        <rdf:type rdf:resource="http://www.w3.org/2003/11/swrl#Variable"/>
    </rdf:Description>
    <rdf:Description rdf:about="urn:swrl:var#doc">
        <rdf:type rdf:resource="http://www.w3.org/2003/11/swrl#Variable"/>
    </rdf:Description>
    <rdf:Description rdf:about="urn:swrl:var#mi">
        <rdf:type rdf:resource="http://www.w3.org/2003/11/swrl#Variable"/>
    </rdf:Description>
    <rdf:Description rdf:about="urn:swrl:var#vep">
        <rdf:type rdf:resource="http://www.w3.org/2003/11/swrl#Variable"/>
    </rdf:Description>
    <rdf:Description rdf:about="urn:swrl:var#uep">
        <rdf:type rdf:resource="http://www.w3.org/2003/11/swrl#Variable"/>
    </rdf:Description>
    <rdf:Description rdf:about="urn:swrl:var#socs">
        <rdf:type rdf:resource="http://www.w3.org/2003/11/swrl#Variable"/>
    </rdf:Description>
    <rdf:Description rdf:about="urn:swrl:var#uocs">
        <rdf:type rdf:resource="http://www.w3.org/2003/11/swrl#Variable"/>
    </rdf:Description>
    <rdf:Description rdf:about="urn:swrl:var#docs">
        <rdf:type rdf:resource="http://www.w3.org/2003/11/swrl#Variable"/>
    </rdf:Description>
    <rdf:Description rdf:about="urn:swrl:var#mis">
        <rdf:type rdf:resource="http://www.w3.org/2003/11/swrl#Variable"/>
    </rdf:Description>
    <rdf:Description rdf:about="urn:swrl:var#veps">
        <rdf:type rdf:resource="http://www.w3.org/2003/11/swrl#Variable"/>
    </rdf:Description>
    <rdf:Description rdf:about="urn:swrl:var#ueps">
        <rdf:type rdf:resource="http://www.w3.org/2003/11/swrl#Variable"/>
    </rdf:Description>
    <rdf:Description rdf:about="urn:swrl:var#prod">
        <rdf:type rdf:resource="http://www.w3.org/2003/11/swrl#Variable"/>
    </rdf:Description>
    <rdf:Description rdf:about="urn:swrl:var#sum">
        <rdf:type rdf:resource="http://www.w3.org/2003/11/swrl#Variable"/>
    </rdf:Description>
    <rdf:Description>
        <rdf:type rdf:resource="http://www.w3.org/2003/11/swrl#Imp"/>
        <swrl:body>
            <rdf:Description>
                <rdf:type rdf:resource="http://www.w3.org/2003/11/swrl#AtomList"/>
                <rdf:first>
                    <rdf:Description>
                        <rdf:type rdf:resource="http://www.w3.org/2003/11/swrl#ClassAtom"/>
                        <swrl:classPredicate rdf:resource="http://www.kracr.iiitd.edu.in/ontology/apple/ActiveAgent"/>
                        <swrl:argument1 rdf:resource="urn:swrl:var#ag"/>
                    </rdf:Description>
                </rdf:first>
                <rdf:rest>
                    <rdf:Description>
                        <rdf:type rdf:resource="http://www.w3.org/2003/11/swrl#AtomList"/>
                        <rdf:first>
                            <rdf:Description>
                                <rdf:type rdf:resource="http://www.w3.org/2003/11/swrl#IndividualPropertyAtom"/>
                                <swrl:propertyPredicate rdf:resource="https://w3id.org/AIRO#hasConsequence"/>
                                <swrl:argument1 rdf:resource="urn:swrl:var#a"/>
                                <swrl:argument2 rdf:resource="urn:swrl:var#c"/>
                            </rdf:Description>
                        </rdf:first>
                        <rdf:rest>
                            <rdf:Description>
                                <rdf:type rdf:resource="http://www.w3.org/2003/11/swrl#AtomList"/>
                                <rdf:first>
                                    <rdf:Description>
                                        <rdf:type rdf:resource="http://www.w3.org/2003/11/swrl#IndividualPropertyAtom"/>
                                        <swrl:propertyPredicate rdf:resource="http://www.kracr.iiitd.edu.in/ontology/apple#hasSeverityOfConsequence"/>
                                        <swrl:argument1 rdf:resource="urn:swrl:var#c"/>
                                        <swrl:argument2 rdf:resource="urn:swrl:var#soc"/>
                                    </rdf:Description>
                                </rdf:first>
                                <rdf:rest>
                                    <rdf:Description>
                                        <rdf:type rdf:resource="http://www.w3.org/2003/11/swrl#AtomList"/>
                                        <rdf:first>
                                            <rdf:Description>
                                                <rdf:type rdf:resource="http://www.w3.org/2003/11/swrl#IndividualPropertyAtom"/>
                                                <swrl:propertyPredicate rdf:resource="http://www.kracr.iiitd.edu.in/ontology/apple#hasUtilityOfConsequence"/>
                                                <swrl:argument1 rdf:resource="urn:swrl:var#c"/>
                                                <swrl:argument2 rdf:resource="urn:swrl:var#uoc"/>
                                            </rdf:Description>
                                        </rdf:first>
                                        <rdf:rest>
                                            <rdf:Description>
                                                <rdf:type rdf:resource="http://www.w3.org/2003/11/swrl#AtomList"/>
                                                <rdf:first>
                                                    <rdf:Description>
                                                        <rdf:type rdf:resource="http://www.w3.org/2003/11/swrl#IndividualPropertyAtom"/>
                                                        <swrl:propertyPredicate rdf:resource="http://www.kracr.iiitd.edu.in/ontology/apple#hasDurationOfConsequence"/>
                                                        <swrl:argument1 rdf:resource="urn:swrl:var#c"/>
                                                        <swrl:argument2 rdf:resource="urn:swrl:var#doc"/>
                                                    </rdf:Description>
                                                </rdf:first>
                                                <rdf:rest>
                                                    <rdf:Description>
                                                        <rdf:type rdf:resource="http://www.w3.org/2003/11/swrl#AtomList"/>
                                                        <rdf:first>
                                                            <rdf:Description>
                                                                <rdf:type rdf:resource="http://www.w3.org/2003/11/swrl#IndividualPropertyAtom"/>
                                                                <swrl:propertyPredicate rdf:resource="http://www.kracr.iiitd.edu.in/ontology/apple/hasMoralIntention"/>
                                                                <swrl:argument1 rdf:resource="urn:swrl:var#ag"/>
                                                                <swrl:argument2 rdf:resource="urn:swrl:var#mi"/>
                                                            </rdf:Description>
                                                        </rdf:first>
                                                        <rdf:rest>
                                                            <rdf:Description>
                                                                <rdf:type rdf:resource="http://www.w3.org/2003/11/swrl#AtomList"/>
                                                                <rdf:first>
                                                                    <rdf:Description>
                                                                        <rdf:type rdf:resource="http://www.w3.org/2003/11/swrl#IndividualPropertyAtom"/>
                                                                        <swrl:propertyPredicate rdf:resource="http://www.kracr.iiitd.edu.in/ontology/apple/violatesEthicalPrinciple"/>
                                                                        <swrl:argument1 rdf:resource="urn:swrl:var#a"/>
                                                                        <swrl:argument2 rdf:resource="urn:swrl:var#vep"/>
                                                                    </rdf:Description>
                                                                </rdf:first>
                                                                <rdf:rest>
                                                                    <rdf:Description>
                                                                        <rdf:type rdf:resource="http://www.w3.org/2003/11/swrl#AtomList"/>
                                                                        <rdf:first>
                                                                            <rdf:Description>
                                                                                <rdf:type rdf:resource="http://www.w3.org/2003/11/swrl#IndividualPropertyAtom"/>
                                                                                <swrl:propertyPredicate rdf:resource="http://www.kracr.iiitd.edu.in/ontology/apple/upholdsEthicalPrinciple"/>
                                                                                <swrl:argument1 rdf:resource="urn:swrl:var#a"/>
                                                                                <swrl:argument2 rdf:resource="urn:swrl:var#uep"/>
                                                                            </rdf:Description>
                                                                        </rdf:first>
                                                                        <rdf:rest>
                                                                            <rdf:Description>
                                                                                <rdf:type rdf:resource="http://www.w3.org/2003/11/swrl#AtomList"/>
                                                                                <rdf:first>
                                                                                    <rdf:Description>
                                                                                        <rdf:type rdf:resource="http://www.w3.org/2003/11/swrl#DatavaluedPropertyAtom"/>
                                                                                        <swrl:propertyPredicate rdf:resource="http://www.kracr.iiitd.edu.in/ontology/apple/hasScore"/>
                                                                                        <swrl:argument1 rdf:resource="urn:swrl:var#soc"/>
                                                                                        <swrl:argument2 rdf:resource="urn:swrl:var#socs"/>
                                                                                    </rdf:Description>
                                                                                </rdf:first>
                                                                                <rdf:rest>
                                                                                    <rdf:Description>
                                                                                        <rdf:type rdf:resource="http://www.w3.org/2003/11/swrl#AtomList"/>
                                                                                        <rdf:first>
                                                                                            <rdf:Description>
                                                                                                <rdf:type rdf:resource="http://www.w3.org/2003/11/swrl#DatavaluedPropertyAtom"/>
                                                                                                <swrl:propertyPredicate rdf:resource="http://www.kracr.iiitd.edu.in/ontology/apple/hasScore"/>
                                                                                                <swrl:argument1 rdf:resource="urn:swrl:var#uoc"/>
                                                                                                <swrl:argument2 rdf:resource="urn:swrl:var#uocs"/>
                                                                                            </rdf:Description>
                                                                                        </rdf:first>
                                                                                        <rdf:rest>
                                                                                            <rdf:Description>
                                                                                                <rdf:type rdf:resource="http://www.w3.org/2003/11/swrl#AtomList"/>
                                                                                                <rdf:first>
                                                                                                    <rdf:Description>
                                                                                                        <rdf:type rdf:resource="http://www.w3.org/2003/11/swrl#DatavaluedPropertyAtom"/>
                                                                                                        <swrl:propertyPredicate rdf:resource="http://www.kracr.iiitd.edu.in/ontology/apple/hasScore"/>
                                                                                                        <swrl:argument1 rdf:resource="urn:swrl:var#doc"/>
                                                                                                        <swrl:argument2 rdf:resource="urn:swrl:var#docs"/>
                                                                                                    </rdf:Description>
                                                                                                </rdf:first>
                                                                                                <rdf:rest>
                                                                                                    <rdf:Description>
                                                                                                        <rdf:type rdf:resource="http://www.w3.org/2003/11/swrl#AtomList"/>
                                                                                                        <rdf:first>
                                                                                                            <rdf:Description>
                                                                                                                <rdf:type rdf:resource="http://www.w3.org/2003/11/swrl#DatavaluedPropertyAtom"/>
                                                                                                                <swrl:propertyPredicate rdf:resource="http://www.kracr.iiitd.edu.in/ontology/apple/hasScore"/>
                                                                                                                <swrl:argument1 rdf:resource="urn:swrl:var#mi"/>
                                                                                                                <swrl:argument2 rdf:resource="urn:swrl:var#mis"/>
                                                                                                            </rdf:Description>
                                                                                                        </rdf:first>
                                                                                                        <rdf:rest>
                                                                                                            <rdf:Description>
                                                                                                                <rdf:type rdf:resource="http://www.w3.org/2003/11/swrl#AtomList"/>
                                                                                                                <rdf:first>
                                                                                                                    <rdf:Description>
                                                                                                                        <rdf:type rdf:resource="http://www.w3.org/2003/11/swrl#DatavaluedPropertyAtom"/>
                                                                                                                        <swrl:propertyPredicate rdf:resource="http://www.kracr.iiitd.edu.in/ontology/apple/hasScore"/>
                                                                                                                        <swrl:argument1 rdf:resource="urn:swrl:var#vep"/>
                                                                                                                        <swrl:argument2 rdf:resource="urn:swrl:var#veps"/>
                                                                                                                    </rdf:Description>
                                                                                                                </rdf:first>
                                                                                                                <rdf:rest>
                                                                                                                    <rdf:Description>
                                                                                                                        <rdf:type rdf:resource="http://www.w3.org/2003/11/swrl#AtomList"/>
                                                                                                                        <rdf:first>
                                                                                                                            <rdf:Description>
                                                                                                                                <rdf:type rdf:resource="http://www.w3.org/2003/11/swrl#DatavaluedPropertyAtom"/>
                                                                                                                                <swrl:propertyPredicate rdf:resource="http://www.kracr.iiitd.edu.in/ontology/apple/hasScore"/>
                                                                                                                                <swrl:argument1 rdf:resource="urn:swrl:var#uep"/>
                                                                                                                                <swrl:argument2 rdf:resource="urn:swrl:var#ueps"/>
                                                                                                                            </rdf:Description>
                                                                                                                        </rdf:first>
                                                                                                                        <rdf:rest>
                                                                                                                            <rdf:Description>
                                                                                                                                <rdf:type rdf:resource="http://www.w3.org/2003/11/swrl#AtomList"/>
                                                                                                                                <rdf:first>
                                                                                                                                    <rdf:Description>
                                                                                                                                        <rdf:type rdf:resource="http://www.w3.org/2003/11/swrl#BuiltinAtom"/>
                                                                                                                                        <swrl:builtin rdf:resource="http://www.w3.org/2003/11/swrlb#multiply"/>
                                                                                                                                        <swrl:arguments rdf:parseType="Collection">
                                                                                                                                            <rdf:Description rdf:about="urn:swrl:var#prod"/>
                                                                                                                                            <rdf:Description rdf:about="urn:swrl:var#socs"/>
                                                                                                                                            <rdf:Description rdf:about="urn:swrl:var#uocs"/>
                                                                                                                                            <rdf:Description rdf:about="urn:swrl:var#docs"/>
                                                                                                                                        </swrl:arguments>
                                                                                                                                    </rdf:Description>
                                                                                                                                </rdf:first>
                                                                                                                                <rdf:rest>
                                                                                                                                    <rdf:Description>
                                                                                                                                        <rdf:type rdf:resource="http://www.w3.org/2003/11/swrl#AtomList"/>
                                                                                                                                        <rdf:first>
                                                                                                                                            <rdf:Description>
                                                                                                                                                <rdf:type rdf:resource="http://www.w3.org/2003/11/swrl#BuiltinAtom"/>
                                                                                                                                                <swrl:builtin rdf:resource="http://www.w3.org/2003/11/swrlb#add"/>
                                                                                                                                                <swrl:arguments rdf:parseType="Collection">
                                                                                                                                                    <rdf:Description rdf:about="urn:swrl:var#sum"/>
                                                                                                                                                    <rdf:Description rdf:about="urn:swrl:var#prod"/>
                                                                                                                                                    <rdf:Description rdf:about="urn:swrl:var#mis"/>
                                                                                                                                                    <rdf:Description rdf:about="urn:swrl:var#veps"/>
                                                                                                                                                    <rdf:Description rdf:about="urn:swrl:var#ueps"/>
                                                                                                                                                </swrl:arguments>
                                                                                                                                            </rdf:Description>
                                                                                                                                        </rdf:first>
                                                                                                                                        <rdf:rest>
                                                                                                                                            <rdf:Description>
                                                                                                                                                <rdf:type rdf:resource="http://www.w3.org/2003/11/swrl#AtomList"/>
                                                                                                                                                <rdf:first>
                                                                                                                                                    <rdf:Description>
                                                                                                                                                        <rdf:type rdf:resource="http://www.w3.org/2003/11/swrl#BuiltinAtom"/>
                                                                                                                                                        <swrl:builtin rdf:resource="http://www.w3.org/2003/11/swrlb#greaterThan"/>
                                                                                                                                                        <swrl:arguments>
                                                                                                                                                            <rdf:Description>
                                                                                                                                                                <rdf:type rdf:resource="http://www.w3.org/1999/02/22-rdf-syntax-ns#List"/>
                                                                                                                                                                <rdf:first rdf:resource="urn:swrl:var#sum"/>
                                                                                                                                                                <rdf:rest>
                                                                                                                                                                    <rdf:Description>
                                                                                                                                                                        <rdf:type rdf:resource="http://www.w3.org/1999/02/22-rdf-syntax-ns#List"/>
                                                                                                                                                                        <rdf:first rdf:datatype="http://www.w3.org/2001/XMLSchema#integer">0</rdf:first>
                                                                                                                                                                        <rdf:rest rdf:resource="http://www.w3.org/1999/02/22-rdf-syntax-ns#nil"/>
                                                                                                                                                                    </rdf:Description>
                                                                                                                                                                </rdf:rest>
                                                                                                                                                            </rdf:Description>
                                                                                                                                                        </swrl:arguments>
                                                                                                                                                    </rdf:Description>
                                                                                                                                                </rdf:first>
                                                                                                                                                <rdf:rest rdf:resource="http://www.w3.org/1999/02/22-rdf-syntax-ns#nil"/>
                                                                                                                                            </rdf:Description>
                                                                                                                                        </rdf:rest>
                                                                                                                                    </rdf:Description>
                                                                                                                                </rdf:rest>
                                                                                                                            </rdf:Description>
                                                                                                                        </rdf:rest>
                                                                                                                    </rdf:Description>
                                                                                                                </rdf:rest>
                                                                                                            </rdf:Description>
                                                                                                        </rdf:rest>
                                                                                                    </rdf:Description>
                                                                                                </rdf:rest>
                                                                                            </rdf:Description>
                                                                                        </rdf:rest>
                                                                                    </rdf:Description>
                                                                                </rdf:rest>
                                                                            </rdf:Description>
                                                                        </rdf:rest>
                                                                    </rdf:Description>
                                                                </rdf:rest>
                                                            </rdf:Description>
                                                        </rdf:rest>
                                                    </rdf:Description>
                                                </rdf:rest>
                                            </rdf:Description>
                                        </rdf:rest>
                                    </rdf:Description>
                                </rdf:rest>
                            </rdf:Description>
                        </rdf:rest>
                    </rdf:Description>
                </rdf:rest>
            </rdf:Description>
        </swrl:body>
        <swrl:head>
            <rdf:Description>
                <rdf:type rdf:resource="http://www.w3.org/2003/11/swrl#AtomList"/>
                <rdf:first>
                    <rdf:Description>
                        <rdf:type rdf:resource="http://www.w3.org/2003/11/swrl#ClassAtom"/>
                        <swrl:classPredicate rdf:resource="http://www.kracr.iiitd.edu.in/ontology/apple/MorallyRightAction"/>
                        <swrl:argument1 rdf:resource="urn:swrl:var#a"/>
                    </rdf:Description>
                </rdf:first>
                <rdf:rest rdf:resource="http://www.w3.org/1999/02/22-rdf-syntax-ns#nil"/>
            </rdf:Description>
        </swrl:head>
    </rdf:Description>
    <rdf:Description>
        <rdf:type rdf:resource="http://www.w3.org/2003/11/swrl#Imp"/>
        <swrl:body>
            <rdf:Description>
                <rdf:type rdf:resource="http://www.w3.org/2003/11/swrl#AtomList"/>
                <rdf:first>
                    <rdf:Description>
                        <rdf:type rdf:resource="http://www.w3.org/2003/11/swrl#ClassAtom"/>
                        <swrl:classPredicate rdf:resource="http://www.kracr.iiitd.edu.in/ontology/apple/ActiveAgent"/>
                        <swrl:argument1 rdf:resource="urn:swrl:var#ag"/>
                    </rdf:Description>
                </rdf:first>
                <rdf:rest>
                    <rdf:Description>
                        <rdf:type rdf:resource="http://www.w3.org/2003/11/swrl#AtomList"/>
                        <rdf:first>
                            <rdf:Description>
                                <rdf:type rdf:resource="http://www.w3.org/2003/11/swrl#IndividualPropertyAtom"/>
                                <swrl:propertyPredicate rdf:resource="https://w3id.org/AIRO#hasConsequence"/>
                                <swrl:argument1 rdf:resource="urn:swrl:var#a"/>
                                <swrl:argument2 rdf:resource="urn:swrl:var#c"/>
                            </rdf:Description>
                        </rdf:first>
                        <rdf:rest>
                            <rdf:Description>
                                <rdf:type rdf:resource="http://www.w3.org/2003/11/swrl#AtomList"/>
                                <rdf:first>
                                    <rdf:Description>
                                        <rdf:type rdf:resource="http://www.w3.org/2003/11/swrl#IndividualPropertyAtom"/>
                                        <swrl:propertyPredicate rdf:resource="http://www.kracr.iiitd.edu.in/ontology/apple#hasSeverityOfConsequence"/>
                                        <swrl:argument1 rdf:resource="urn:swrl:var#c"/>
                                        <swrl:argument2 rdf:resource="urn:swrl:var#soc"/>
                                    </rdf:Description>
                                </rdf:first>
                                <rdf:rest>
                                    <rdf:Description>
                                        <rdf:type rdf:resource="http://www.w3.org/2003/11/swrl#AtomList"/>
                                        <rdf:first>
                                            <rdf:Description>
                                                <rdf:type rdf:resource="http://www.w3.org/2003/11/swrl#IndividualPropertyAtom"/>
                                                <swrl:propertyPredicate rdf:resource="http://www.kracr.iiitd.edu.in/ontology/apple#hasUtilityOfConsequence"/>
                                                <swrl:argument1 rdf:resource="urn:swrl:var#c"/>
                                                <swrl:argument2 rdf:resource="urn:swrl:var#uoc"/>
                                            </rdf:Description>
                                        </rdf:first>
                                        <rdf:rest>
                                            <rdf:Description>
                                                <rdf:type rdf:resource="http://www.w3.org/2003/11/swrl#AtomList"/>
                                                <rdf:first>
                                                    <rdf:Description>
                                                        <rdf:type rdf:resource="http://www.w3.org/2003/11/swrl#IndividualPropertyAtom"/>
                                                        <swrl:propertyPredicate rdf:resource="http://www.kracr.iiitd.edu.in/ontology/apple#hasDurationOfConsequence"/>
                                                        <swrl:argument1 rdf:resource="urn:swrl:var#c"/>
                                                        <swrl:argument2 rdf:resource="urn:swrl:var#doc"/>
                                                    </rdf:Description>
                                                </rdf:first>
                                                <rdf:rest>
                                                    <rdf:Description>
                                                        <rdf:type rdf:resource="http://www.w3.org/2003/11/swrl#AtomList"/>
                                                        <rdf:first>
                                                            <rdf:Description>
                                                                <rdf:type rdf:resource="http://www.w3.org/2003/11/swrl#IndividualPropertyAtom"/>
                                                                <swrl:propertyPredicate rdf:resource="http://www.kracr.iiitd.edu.in/ontology/apple/hasMoralIntention"/>
                                                                <swrl:argument1 rdf:resource="urn:swrl:var#ag"/>
                                                                <swrl:argument2 rdf:resource="urn:swrl:var#mi"/>
                                                            </rdf:Description>
                                                        </rdf:first>
                                                        <rdf:rest>
                                                            <rdf:Description>
                                                                <rdf:type rdf:resource="http://www.w3.org/2003/11/swrl#AtomList"/>
                                                                <rdf:first>
                                                                    <rdf:Description>
                                                                        <rdf:type rdf:resource="http://www.w3.org/2003/11/swrl#IndividualPropertyAtom"/>
                                                                        <swrl:propertyPredicate rdf:resource="http://www.kracr.iiitd.edu.in/ontology/apple/violatesEthicalPrinciple"/>
                                                                        <swrl:argument1 rdf:resource="urn:swrl:var#a"/>
                                                                        <swrl:argument2 rdf:resource="urn:swrl:var#vep"/>
                                                                    </rdf:Description>
                                                                </rdf:first>
                                                                <rdf:rest>
                                                                    <rdf:Description>
                                                                        <rdf:type rdf:resource="http://www.w3.org/2003/11/swrl#AtomList"/>
                                                                        <rdf:first>
                                                                            <rdf:Description>
                                                                                <rdf:type rdf:resource="http://www.w3.org/2003/11/swrl#IndividualPropertyAtom"/>
                                                                                <swrl:propertyPredicate rdf:resource="http://www.kracr.iiitd.edu.in/ontology/apple/upholdsEthicalPrinciple"/>
                                                                                <swrl:argument1 rdf:resource="urn:swrl:var#a"/>
                                                                                <swrl:argument2 rdf:resource="urn:swrl:var#uep"/>
                                                                            </rdf:Description>
                                                                        </rdf:first>
                                                                        <rdf:rest>
                                                                            <rdf:Description>
                                                                                <rdf:type rdf:resource="http://www.w3.org/2003/11/swrl#AtomList"/>
                                                                                <rdf:first>
                                                                                    <rdf:Description>
                                                                                        <rdf:type rdf:resource="http://www.w3.org/2003/11/swrl#DatavaluedPropertyAtom"/>
                                                                                        <swrl:propertyPredicate rdf:resource="http://www.kracr.iiitd.edu.in/ontology/apple/hasScore"/>
                                                                                        <swrl:argument1 rdf:resource="urn:swrl:var#soc"/>
                                                                                        <swrl:argument2 rdf:resource="urn:swrl:var#socs"/>
                                                                                    </rdf:Description>
                                                                                </rdf:first>
                                                                                <rdf:rest>
                                                                                    <rdf:Description>
                                                                                        <rdf:type rdf:resource="http://www.w3.org/2003/11/swrl#AtomList"/>
                                                                                        <rdf:first>
                                                                                            <rdf:Description>
                                                                                                <rdf:type rdf:resource="http://www.w3.org/2003/11/swrl#DatavaluedPropertyAtom"/>
                                                                                                <swrl:propertyPredicate rdf:resource="http://www.kracr.iiitd.edu.in/ontology/apple/hasScore"/>
                                                                                                <swrl:argument1 rdf:resource="urn:swrl:var#uoc"/>
                                                                                                <swrl:argument2 rdf:resource="urn:swrl:var#uocs"/>
                                                                                            </rdf:Description>
                                                                                        </rdf:first>
                                                                                        <rdf:rest>
                                                                                            <rdf:Description>
                                                                                                <rdf:type rdf:resource="http://www.w3.org/2003/11/swrl#AtomList"/>
                                                                                                <rdf:first>
                                                                                                    <rdf:Description>
                                                                                                        <rdf:type rdf:resource="http://www.w3.org/2003/11/swrl#DatavaluedPropertyAtom"/>
                                                                                                        <swrl:propertyPredicate rdf:resource="http://www.kracr.iiitd.edu.in/ontology/apple/hasScore"/>
                                                                                                        <swrl:argument1 rdf:resource="urn:swrl:var#doc"/>
                                                                                                        <swrl:argument2 rdf:resource="urn:swrl:var#docs"/>
                                                                                                    </rdf:Description>
                                                                                                </rdf:first>
                                                                                                <rdf:rest>
                                                                                                    <rdf:Description>
                                                                                                        <rdf:type rdf:resource="http://www.w3.org/2003/11/swrl#AtomList"/>
                                                                                                        <rdf:first>
                                                                                                            <rdf:Description>
                                                                                                                <rdf:type rdf:resource="http://www.w3.org/2003/11/swrl#DatavaluedPropertyAtom"/>
                                                                                                                <swrl:propertyPredicate rdf:resource="http://www.kracr.iiitd.edu.in/ontology/apple/hasScore"/>
                                                                                                                <swrl:argument1 rdf:resource="urn:swrl:var#mi"/>
                                                                                                                <swrl:argument2 rdf:resource="urn:swrl:var#mis"/>
                                                                                                            </rdf:Description>
                                                                                                        </rdf:first>
                                                                                                        <rdf:rest>
                                                                                                            <rdf:Description>
                                                                                                                <rdf:type rdf:resource="http://www.w3.org/2003/11/swrl#AtomList"/>
                                                                                                                <rdf:first>
                                                                                                                    <rdf:Description>
                                                                                                                        <rdf:type rdf:resource="http://www.w3.org/2003/11/swrl#DatavaluedPropertyAtom"/>
                                                                                                                        <swrl:propertyPredicate rdf:resource="http://www.kracr.iiitd.edu.in/ontology/apple/hasScore"/>
                                                                                                                        <swrl:argument1 rdf:resource="urn:swrl:var#vep"/>
                                                                                                                        <swrl:argument2 rdf:resource="urn:swrl:var#veps"/>
                                                                                                                    </rdf:Description>
                                                                                                                </rdf:first>
                                                                                                                <rdf:rest>
                                                                                                                    <rdf:Description>
                                                                                                                        <rdf:type rdf:resource="http://www.w3.org/2003/11/swrl#AtomList"/>
                                                                                                                        <rdf:first>
                                                                                                                            <rdf:Description>
                                                                                                                                <rdf:type rdf:resource="http://www.w3.org/2003/11/swrl#DatavaluedPropertyAtom"/>
                                                                                                                                <swrl:propertyPredicate rdf:resource="http://www.kracr.iiitd.edu.in/ontology/apple/hasScore"/>
                                                                                                                                <swrl:argument1 rdf:resource="urn:swrl:var#uep"/>
                                                                                                                                <swrl:argument2 rdf:resource="urn:swrl:var#ueps"/>
                                                                                                                            </rdf:Description>
                                                                                                                        </rdf:first>
                                                                                                                        <rdf:rest>
                                                                                                                            <rdf:Description>
                                                                                                                                <rdf:type rdf:resource="http://www.w3.org/2003/11/swrl#AtomList"/>
                                                                                                                                <rdf:first>
                                                                                                                                    <rdf:Description>
                                                                                                                                        <rdf:type rdf:resource="http://www.w3.org/2003/11/swrl#BuiltinAtom"/>
                                                                                                                                        <swrl:builtin rdf:resource="http://www.w3.org/2003/11/swrlb#multiply"/>
                                                                                                                                        <swrl:arguments rdf:parseType="Collection">
                                                                                                                                            <rdf:Description rdf:about="urn:swrl:var#prod"/>
                                                                                                                                            <rdf:Description rdf:about="urn:swrl:var#socs"/>
                                                                                                                                            <rdf:Description rdf:about="urn:swrl:var#uocs"/>
                                                                                                                                            <rdf:Description rdf:about="urn:swrl:var#docs"/>
                                                                                                                                        </swrl:arguments>
                                                                                                                                    </rdf:Description>
                                                                                                                                </rdf:first>
                                                                                                                                <rdf:rest>
                                                                                                                                    <rdf:Description>
                                                                                                                                        <rdf:type rdf:resource="http://www.w3.org/2003/11/swrl#AtomList"/>
                                                                                                                                        <rdf:first>
                                                                                                                                            <rdf:Description>
                                                                                                                                                <rdf:type rdf:resource="http://www.w3.org/2003/11/swrl#BuiltinAtom"/>
                                                                                                                                                <swrl:builtin rdf:resource="http://www.w3.org/2003/11/swrlb#add"/>
                                                                                                                                                <swrl:arguments rdf:parseType="Collection">
                                                                                                                                                    <rdf:Description rdf:about="urn:swrl:var#sum"/>
                                                                                                                                                    <rdf:Description rdf:about="urn:swrl:var#prod"/>
                                                                                                                                                    <rdf:Description rdf:about="urn:swrl:var#mis"/>
                                                                                                                                                    <rdf:Description rdf:about="urn:swrl:var#veps"/>
                                                                                                                                                    <rdf:Description rdf:about="urn:swrl:var#ueps"/>
                                                                                                                                                </swrl:arguments>
                                                                                                                                            </rdf:Description>
                                                                                                                                        </rdf:first>
                                                                                                                                        <rdf:rest>
                                                                                                                                            <rdf:Description>
                                                                                                                                                <rdf:type rdf:resource="http://www.w3.org/2003/11/swrl#AtomList"/>
                                                                                                                                                <rdf:first>
                                                                                                                                                    <rdf:Description>
                                                                                                                                                        <rdf:type rdf:resource="http://www.w3.org/2003/11/swrl#BuiltinAtom"/>
                                                                                                                                                        <swrl:builtin rdf:resource="http://www.w3.org/2003/11/swrlb#lessThan"/>
                                                                                                                                                        <swrl:arguments>
                                                                                                                                                            <rdf:Description>
                                                                                                                                                                <rdf:type rdf:resource="http://www.w3.org/1999/02/22-rdf-syntax-ns#List"/>
                                                                                                                                                                <rdf:first rdf:resource="urn:swrl:var#sum"/>
                                                                                                                                                                <rdf:rest>
                                                                                                                                                                    <rdf:Description>
                                                                                                                                                                        <rdf:type rdf:resource="http://www.w3.org/1999/02/22-rdf-syntax-ns#List"/>
                                                                                                                                                                        <rdf:first rdf:datatype="http://www.w3.org/2001/XMLSchema#integer">0</rdf:first>
                                                                                                                                                                        <rdf:rest rdf:resource="http://www.w3.org/1999/02/22-rdf-syntax-ns#nil"/>
                                                                                                                                                                    </rdf:Description>
                                                                                                                                                                </rdf:rest>
                                                                                                                                                            </rdf:Description>
                                                                                                                                                        </swrl:arguments>
                                                                                                                                                    </rdf:Description>
                                                                                                                                                </rdf:first>
                                                                                                                                                <rdf:rest rdf:resource="http://www.w3.org/1999/02/22-rdf-syntax-ns#nil"/>
                                                                                                                                            </rdf:Description>
                                                                                                                                        </rdf:rest>
                                                                                                                                    </rdf:Description>
                                                                                                                                </rdf:rest>
                                                                                                                            </rdf:Description>
                                                                                                                        </rdf:rest>
                                                                                                                    </rdf:Description>
                                                                                                                </rdf:rest>
                                                                                                            </rdf:Description>
                                                                                                        </rdf:rest>
                                                                                                    </rdf:Description>
                                                                                                </rdf:rest>
                                                                                            </rdf:Description>
                                                                                        </rdf:rest>
                                                                                    </rdf:Description>
                                                                                </rdf:rest>
                                                                            </rdf:Description>
                                                                        </rdf:rest>
                                                                    </rdf:Description>
                                                                </rdf:rest>
                                                            </rdf:Description>
                                                        </rdf:rest>
                                                    </rdf:Description>
                                                </rdf:rest>
                                            </rdf:Description>
                                        </rdf:rest>
                                    </rdf:Description>
                                </rdf:rest>
                            </rdf:Description>
                        </rdf:rest>
                    </rdf:Description>
                </rdf:rest>
            </rdf:Description>
        </swrl:body>
        <swrl:head>
            <rdf:Description>
                <rdf:type rdf:resource="http://www.w3.org/2003/11/swrl#AtomList"/>
                <rdf:first>
                    <rdf:Description>
                        <rdf:type rdf:resource="http://www.w3.org/2003/11/swrl#ClassAtom"/>
                        <swrl:classPredicate rdf:resource="http://www.kracr.iiitd.edu.in/ontology/apple/MorallyWrongAction"/>
                        <swrl:argument1 rdf:resource="urn:swrl:var#a"/>
                    </rdf:Description>
                </rdf:first>
                <rdf:rest rdf:resource="http://www.w3.org/1999/02/22-rdf-syntax-ns#nil"/>
            </rdf:Description>
        </swrl:head>
    </rdf:Description>
    <rdf:Description>
        <rdf:type rdf:resource="http://www.w3.org/2003/11/swrl#Imp"/>
        <swrl:body>
            <rdf:Description>
                <rdf:type rdf:resource="http://www.w3.org/2003/11/swrl#AtomList"/>
                <rdf:first>
                    <rdf:Description>
                        <rdf:type rdf:resource="http://www.w3.org/2003/11/swrl#ClassAtom"/>
                        <swrl:classPredicate rdf:resource="http://www.kracr.iiitd.edu.in/ontology/apple/ActiveAgent"/>
                        <swrl:argument1 rdf:resource="urn:swrl:var#ag"/>
                    </rdf:Description>
                </rdf:first>
                <rdf:rest>
                    <rdf:Description>
                        <rdf:type rdf:resource="http://www.w3.org/2003/11/swrl#AtomList"/>
                        <rdf:first>
                            <rdf:Description>
                                <rdf:type rdf:resource="http://www.w3.org/2003/11/swrl#IndividualPropertyAtom"/>
                                <swrl:propertyPredicate rdf:resource="https://w3id.org/AIRO#hasConsequence"/>
                                <swrl:argument1 rdf:resource="urn:swrl:var#a"/>
                                <swrl:argument2 rdf:resource="urn:swrl:var#c"/>
                            </rdf:Description>
                        </rdf:first>
                        <rdf:rest>
                            <rdf:Description>
                                <rdf:type rdf:resource="http://www.w3.org/2003/11/swrl#AtomList"/>
                                <rdf:first>
                                    <rdf:Description>
                                        <rdf:type rdf:resource="http://www.w3.org/2003/11/swrl#IndividualPropertyAtom"/>
                                        <swrl:propertyPredicate rdf:resource="http://www.kracr.iiitd.edu.in/ontology/apple#hasSeverityOfConsequence"/>
                                        <swrl:argument1 rdf:resource="urn:swrl:var#c"/>
                                        <swrl:argument2 rdf:resource="urn:swrl:var#soc"/>
                                    </rdf:Description>
                                </rdf:first>
                                <rdf:rest>
                                    <rdf:Description>
                                        <rdf:type rdf:resource="http://www.w3.org/2003/11/swrl#AtomList"/>
                                        <rdf:first>
                                            <rdf:Description>
                                                <rdf:type rdf:resource="http://www.w3.org/2003/11/swrl#IndividualPropertyAtom"/>
                                                <swrl:propertyPredicate rdf:resource="http://www.kracr.iiitd.edu.in/ontology/apple#hasUtilityOfConsequence"/>
                                                <swrl:argument1 rdf:resource="urn:swrl:var#c"/>
                                                <swrl:argument2 rdf:resource="urn:swrl:var#uoc"/>
                                            </rdf:Description>
                                        </rdf:first>
                                        <rdf:rest>
                                            <rdf:Description>
                                                <rdf:type rdf:resource="http://www.w3.org/2003/11/swrl#AtomList"/>
                                                <rdf:first>
                                                    <rdf:Description>
                                                        <rdf:type rdf:resource="http://www.w3.org/2003/11/swrl#IndividualPropertyAtom"/>
                                                        <swrl:propertyPredicate rdf:resource="http://www.kracr.iiitd.edu.in/ontology/apple#hasDurationOfConsequence"/>
                                                        <swrl:argument1 rdf:resource="urn:swrl:var#c"/>
                                                        <swrl:argument2 rdf:resource="urn:swrl:var#doc"/>
                                                    </rdf:Description>
                                                </rdf:first>
                                                <rdf:rest>
                                                    <rdf:Description>
                                                        <rdf:type rdf:resource="http://www.w3.org/2003/11/swrl#AtomList"/>
                                                        <rdf:first>
                                                            <rdf:Description>
                                                                <rdf:type rdf:resource="http://www.w3.org/2003/11/swrl#IndividualPropertyAtom"/>
                                                                <swrl:propertyPredicate rdf:resource="http://www.kracr.iiitd.edu.in/ontology/apple/hasMoralIntention"/>
                                                                <swrl:argument1 rdf:resource="urn:swrl:var#ag"/>
                                                                <swrl:argument2 rdf:resource="urn:swrl:var#mi"/>
                                                            </rdf:Description>
                                                        </rdf:first>
                                                        <rdf:rest>
                                                            <rdf:Description>
                                                                <rdf:type rdf:resource="http://www.w3.org/2003/11/swrl#AtomList"/>
                                                                <rdf:first>
                                                                    <rdf:Description>
                                                                        <rdf:type rdf:resource="http://www.w3.org/2003/11/swrl#IndividualPropertyAtom"/>
                                                                        <swrl:propertyPredicate rdf:resource="http://www.kracr.iiitd.edu.in/ontology/apple/violatesEthicalPrinciple"/>
                                                                        <swrl:argument1 rdf:resource="urn:swrl:var#a"/>
                                                                        <swrl:argument2 rdf:resource="urn:swrl:var#vep"/>
                                                                    </rdf:Description>
                                                                </rdf:first>
                                                                <rdf:rest>
                                                                    <rdf:Description>
                                                                        <rdf:type rdf:resource="http://www.w3.org/2003/11/swrl#AtomList"/>
                                                                        <rdf:first>
                                                                            <rdf:Description>
                                                                                <rdf:type rdf:resource="http://www.w3.org/2003/11/swrl#IndividualPropertyAtom"/>
                                                                                <swrl:propertyPredicate rdf:resource="http://www.kracr.iiitd.edu.in/ontology/apple/upholdsEthicalPrinciple"/>
                                                                                <swrl:argument1 rdf:resource="urn:swrl:var#a"/>
                                                                                <swrl:argument2 rdf:resource="urn:swrl:var#uep"/>
                                                                            </rdf:Description>
                                                                        </rdf:first>
                                                                        <rdf:rest>
                                                                            <rdf:Description>
                                                                                <rdf:type rdf:resource="http://www.w3.org/2003/11/swrl#AtomList"/>
                                                                                <rdf:first>
                                                                                    <rdf:Description>
                                                                                        <rdf:type rdf:resource="http://www.w3.org/2003/11/swrl#DatavaluedPropertyAtom"/>
                                                                                        <swrl:propertyPredicate rdf:resource="http://www.kracr.iiitd.edu.in/ontology/apple/hasScore"/>
                                                                                        <swrl:argument1 rdf:resource="urn:swrl:var#soc"/>
                                                                                        <swrl:argument2 rdf:resource="urn:swrl:var#socs"/>
                                                                                    </rdf:Description>
                                                                                </rdf:first>
                                                                                <rdf:rest>
                                                                                    <rdf:Description>
                                                                                        <rdf:type rdf:resource="http://www.w3.org/2003/11/swrl#AtomList"/>
                                                                                        <rdf:first>
                                                                                            <rdf:Description>
                                                                                                <rdf:type rdf:resource="http://www.w3.org/2003/11/swrl#DatavaluedPropertyAtom"/>
                                                                                                <swrl:propertyPredicate rdf:resource="http://www.kracr.iiitd.edu.in/ontology/apple/hasScore"/>
                                                                                                <swrl:argument1 rdf:resource="urn:swrl:var#uoc"/>
                                                                                                <swrl:argument2 rdf:resource="urn:swrl:var#uocs"/>
                                                                                            </rdf:Description>
                                                                                        </rdf:first>
                                                                                        <rdf:rest>
                                                                                            <rdf:Description>
                                                                                                <rdf:type rdf:resource="http://www.w3.org/2003/11/swrl#AtomList"/>
                                                                                                <rdf:first>
                                                                                                    <rdf:Description>
                                                                                                        <rdf:type rdf:resource="http://www.w3.org/2003/11/swrl#DatavaluedPropertyAtom"/>
                                                                                                        <swrl:propertyPredicate rdf:resource="http://www.kracr.iiitd.edu.in/ontology/apple/hasScore"/>
                                                                                                        <swrl:argument1 rdf:resource="urn:swrl:var#doc"/>
                                                                                                        <swrl:argument2 rdf:resource="urn:swrl:var#docs"/>
                                                                                                    </rdf:Description>
                                                                                                </rdf:first>
                                                                                                <rdf:rest>
                                                                                                    <rdf:Description>
                                                                                                        <rdf:type rdf:resource="http://www.w3.org/2003/11/swrl#AtomList"/>
                                                                                                        <rdf:first>
                                                                                                            <rdf:Description>
                                                                                                                <rdf:type rdf:resource="http://www.w3.org/2003/11/swrl#DatavaluedPropertyAtom"/>
                                                                                                                <swrl:propertyPredicate rdf:resource="http://www.kracr.iiitd.edu.in/ontology/apple/hasScore"/>
                                                                                                                <swrl:argument1 rdf:resource="urn:swrl:var#mi"/>
                                                                                                                <swrl:argument2 rdf:resource="urn:swrl:var#mis"/>
                                                                                                            </rdf:Description>
                                                                                                        </rdf:first>
                                                                                                        <rdf:rest>
                                                                                                            <rdf:Description>
                                                                                                                <rdf:type rdf:resource="http://www.w3.org/2003/11/swrl#AtomList"/>
                                                                                                                <rdf:first>
                                                                                                                    <rdf:Description>
                                                                                                                        <rdf:type rdf:resource="http://www.w3.org/2003/11/swrl#DatavaluedPropertyAtom"/>
                                                                                                                        <swrl:propertyPredicate rdf:resource="http://www.kracr.iiitd.edu.in/ontology/apple/hasScore"/>
                                                                                                                        <swrl:argument1 rdf:resource="urn:swrl:var#vep"/>
                                                                                                                        <swrl:argument2 rdf:resource="urn:swrl:var#veps"/>
                                                                                                                    </rdf:Description>
                                                                                                                </rdf:first>
                                                                                                                <rdf:rest>
                                                                                                                    <rdf:Description>
                                                                                                                        <rdf:type rdf:resource="http://www.w3.org/2003/11/swrl#AtomList"/>
                                                                                                                        <rdf:first>
                                                                                                                            <rdf:Description>
                                                                                                                                <rdf:type rdf:resource="http://www.w3.org/2003/11/swrl#DatavaluedPropertyAtom"/>
                                                                                                                                <swrl:propertyPredicate rdf:resource="http://www.kracr.iiitd.edu.in/ontology/apple/hasScore"/>
                                                                                                                                <swrl:argument1 rdf:resource="urn:swrl:var#uep"/>
                                                                                                                                <swrl:argument2 rdf:resource="urn:swrl:var#ueps"/>
                                                                                                                            </rdf:Description>
                                                                                                                        </rdf:first>
                                                                                                                        <rdf:rest>
                                                                                                                            <rdf:Description>
                                                                                                                                <rdf:type rdf:resource="http://www.w3.org/2003/11/swrl#AtomList"/>
                                                                                                                                <rdf:first>
                                                                                                                                    <rdf:Description>
                                                                                                                                        <rdf:type rdf:resource="http://www.w3.org/2003/11/swrl#BuiltinAtom"/>
                                                                                                                                        <swrl:builtin rdf:resource="http://www.w3.org/2003/11/swrlb#multiply"/>
                                                                                                                                        <swrl:arguments rdf:parseType="Collection">
                                                                                                                                            <rdf:Description rdf:about="urn:swrl:var#prod"/>
                                                                                                                                            <rdf:Description rdf:about="urn:swrl:var#socs"/>
                                                                                                                                            <rdf:Description rdf:about="urn:swrl:var#uocs"/>
                                                                                                                                            <rdf:Description rdf:about="urn:swrl:var#docs"/>
                                                                                                                                        </swrl:arguments>
                                                                                                                                    </rdf:Description>
                                                                                                                                </rdf:first>
                                                                                                                                <rdf:rest>
                                                                                                                                    <rdf:Description>
                                                                                                                                        <rdf:type rdf:resource="http://www.w3.org/2003/11/swrl#AtomList"/>
                                                                                                                                        <rdf:first>
                                                                                                                                            <rdf:Description>
                                                                                                                                                <rdf:type rdf:resource="http://www.w3.org/2003/11/swrl#BuiltinAtom"/>
                                                                                                                                                <swrl:builtin rdf:resource="http://www.w3.org/2003/11/swrlb#add"/>
                                                                                                                                                <swrl:arguments rdf:parseType="Collection">
                                                                                                                                                    <rdf:Description rdf:about="urn:swrl:var#sum"/>
                                                                                                                                                    <rdf:Description rdf:about="urn:swrl:var#prod"/>
                                                                                                                                                    <rdf:Description rdf:about="urn:swrl:var#mis"/>
                                                                                                                                                    <rdf:Description rdf:about="urn:swrl:var#veps"/>
                                                                                                                                                    <rdf:Description rdf:about="urn:swrl:var#ueps"/>
                                                                                                                                                </swrl:arguments>
                                                                                                                                            </rdf:Description>
                                                                                                                                        </rdf:first>
                                                                                                                                        <rdf:rest>
                                                                                                                                            <rdf:Description>
                                                                                                                                                <rdf:type rdf:resource="http://www.w3.org/2003/11/swrl#AtomList"/>
                                                                                                                                                <rdf:first>
                                                                                                                                                    <rdf:Description>
                                                                                                                                                        <rdf:type rdf:resource="http://www.w3.org/2003/11/swrl#BuiltinAtom"/>
                                                                                                                                                        <swrl:builtin rdf:resource="http://www.w3.org/2003/11/swrlb#equal"/>
                                                                                                                                                        <swrl:arguments>
                                                                                                                                                            <rdf:Description>
                                                                                                                                                                <rdf:type rdf:resource="http://www.w3.org/1999/02/22-rdf-syntax-ns#List"/>
                                                                                                                                                                <rdf:first rdf:resource="urn:swrl:var#sum"/>
                                                                                                                                                                <rdf:rest>
                                                                                                                                                                    <rdf:Description>
                                                                                                                                                                        <rdf:type rdf:resource="http://www.w3.org/1999/02/22-rdf-syntax-ns#List"/>
                                                                                                                                                                        <rdf:first rdf:datatype="http://www.w3.org/2001/XMLSchema#integer">0</rdf:first>
                                                                                                                                                                        <rdf:rest rdf:resource="http://www.w3.org/1999/02/22-rdf-syntax-ns#nil"/>
                                                                                                                                                                    </rdf:Description>
                                                                                                                                                                </rdf:rest>
                                                                                                                                                            </rdf:Description>
                                                                                                                                                        </swrl:arguments>
                                                                                                                                                    </rdf:Description>
                                                                                                                                                </rdf:first>
                                                                                                                                                <rdf:rest rdf:resource="http://www.w3.org/1999/02/22-rdf-syntax-ns#nil"/>
                                                                                                                                            </rdf:Description>
                                                                                                                                        </rdf:rest>
                                                                                                                                    </rdf:Description>
                                                                                                                                </rdf:rest>
                                                                                                                            </rdf:Description>
                                                                                                                        </rdf:rest>
                                                                                                                    </rdf:Description>
                                                                                                                </rdf:rest>
                                                                                                            </rdf:Description>
                                                                                                        </rdf:rest>
                                                                                                    </rdf:Description>
                                                                                                </rdf:rest>
                                                                                            </rdf:Description>
                                                                                        </rdf:rest>
                                                                                    </rdf:Description>
                                                                                </rdf:rest>
                                                                            </rdf:Description>
                                                                        </rdf:rest>
                                                                    </rdf:Description>
                                                                </rdf:rest>
                                                            </rdf:Description>
                                                        </rdf:rest>
                                                    </rdf:Description>
                                                </rdf:rest>
                                            </rdf:Description>
                                        </rdf:rest>
                                    </rdf:Description>
                                </rdf:rest>
                            </rdf:Description>
                        </rdf:rest>
                    </rdf:Description>
                </rdf:rest>
            </rdf:Description>
        </swrl:body>
        <swrl:head>
            <rdf:Description>
                <rdf:type rdf:resource="http://www.w3.org/2003/11/swrl#AtomList"/>
                <rdf:first>
                    <rdf:Description>
                        <rdf:type rdf:resource="http://www.w3.org/2003/11/swrl#ClassAtom"/>
                        <swrl:classPredicate rdf:resource="http://www.kracr.iiitd.edu.in/ontology/apple/MorallyGreyAction"/>
                        <swrl:argument1 rdf:resource="urn:swrl:var#a"/>
                    </rdf:Description>
                </rdf:first>
                <rdf:rest rdf:resource="http://www.w3.org/1999/02/22-rdf-syntax-ns#nil"/>
            </rdf:Description>
        </swrl:head>
    </rdf:Description>
</rdf:RDF>



<!-- Generated by the OWL API (version 4.5.9.2019-02-01T07:24:44Z) https://github.com/owlcs/owlapi -->

